<?xml version="1.0" encoding="UTF-8"?>
<rdf:RDF xmlns:rdfs="http://www.w3.org/2000/01/rdf-schema#"
         xmlns:rdf="http://www.w3.org/1999/02/22-rdf-syntax-ns#"
         xmlns:skos="http://www.w3.org/2004/02/skos/core#"
         xmlns:dc="http://purl.org/dc/elements/1.1/"
         xmlns:dcterms="http://purl.org/dc/terms/">

   <rdf:Description rdf:about="http://104.244.76.201/Bionet-ANDS-test/schema">
      <rdf:type rdf:resource="http://www.w3.org/2004/02/skos/core#ConceptScheme"/>
      <rdfs:label xml:lang="en">Bionet Species Sighting Standard (RB test v3)</rdfs:label>
      <dcterms:title xml:lang="en">Bionet Species Sighting Standard (RB test v3)</dcterms:title>
      <dcterms:description xml:lang="en">For more information about the Bionet Species Sighting Standard, see https://data.bionet.nsw.gov.au/resources/bionet/BioNet-species-sighting-web-service-data-standard.pdf</dcterms:description>
      <dcterms:subject xml:lang="en">species</dcterms:subject>
      <dcterms:creator>Bionet (NSW Office of Environment and Heritage)</dcterms:creator>
      <dcterms:contributor>Bionet (NSW Office of Environment and Heritage)</dcterms:contributor>
      <dcterms:publisher>Bionet (NSW Office of Environment and Heritage)</dcterms:publisher>
      <skos:hasTopConcept rdf:resource="http://104.244.76.201/Bionet-ANDS-test/schema/d1e2a1900"/>
      <skos:hasTopConcept rdf:resource="http://104.244.76.201/Bionet-ANDS-test/schema/d1e223a1900"/>
      <skos:hasTopConcept rdf:resource="http://104.244.76.201/Bionet-ANDS-test/schema/d1e494a1900"/>
      <skos:hasTopConcept rdf:resource="http://104.244.76.201/Bionet-ANDS-test/schema/d1e661a1900"/>
      <skos:hasTopConcept rdf:resource="http://104.244.76.201/Bionet-ANDS-test/schema/d1e764a1900"/>
      <skos:hasTopConcept rdf:resource="http://104.244.76.201/Bionet-ANDS-test/schema/d1e840a1900"/>
   </rdf:Description>

   <rdf:Description rdf:about="http://104.244.76.201/Bionet-ANDS-test/schema/d1e2a1900">
      <rdf:type rdf:resource="http://www.w3.org/2004/02/skos/core#Concept"/>
      <skos:prefLabel xml:lang="en">Record-level terms</skos:prefLabel>
      <dcterms:creator>Bionet (NSW Office of Environment and Heritage)</dcterms:creator>
      <dcterms:contributor>Bionet (NSW Office of Environment and Heritage)</dcterms:contributor>
      <skos:topConceptOf rdf:resource="http://104.244.76.201/Bionet-ANDS-test/schema"/>
      <skos:narrower rdf:resource="http://104.244.76.201/Bionet-ANDS-test/schema/d1e3a1900"/>
      <skos:narrower rdf:resource="http://104.244.76.201/Bionet-ANDS-test/schema/d1e10a1900"/>
      <skos:narrower rdf:resource="http://104.244.76.201/Bionet-ANDS-test/schema/d1e17a1900"/>
      <skos:narrower rdf:resource="http://104.244.76.201/Bionet-ANDS-test/schema/d1e34a1900"/>
      <skos:narrower rdf:resource="http://104.244.76.201/Bionet-ANDS-test/schema/d1e39a1900"/>
      <skos:narrower rdf:resource="http://104.244.76.201/Bionet-ANDS-test/schema/d1e44a1900"/>
      <skos:narrower rdf:resource="http://104.244.76.201/Bionet-ANDS-test/schema/d1e53a1900"/>
      <skos:narrower rdf:resource="http://104.244.76.201/Bionet-ANDS-test/schema/d1e58a1900"/>
      <skos:narrower rdf:resource="http://104.244.76.201/Bionet-ANDS-test/schema/d1e65a1900"/>
      <skos:narrower rdf:resource="http://104.244.76.201/Bionet-ANDS-test/schema/d1e70a1900"/>
      <skos:narrower rdf:resource="http://104.244.76.201/Bionet-ANDS-test/schema/d1e75a1900"/>
      <skos:narrower rdf:resource="http://104.244.76.201/Bionet-ANDS-test/schema/d1e81a1900"/>
      <skos:narrower rdf:resource="http://104.244.76.201/Bionet-ANDS-test/schema/d1e88a1900"/>
      <skos:narrower rdf:resource="http://104.244.76.201/Bionet-ANDS-test/schema/d1e93a1900"/>
      <skos:narrower rdf:resource="http://104.244.76.201/Bionet-ANDS-test/schema/d1e98a1900"/>
   </rdf:Description>

   <rdf:Description rdf:about="http://104.244.76.201/Bionet-ANDS-test/schema/d1e223a1900">
      <rdf:type rdf:resource="http://www.w3.org/2004/02/skos/core#Concept"/>
      <skos:prefLabel xml:lang="en">Occurrence</skos:prefLabel>
      <dcterms:creator>Bionet (NSW Office of Environment and Heritage)</dcterms:creator>
      <dcterms:contributor>Bionet (NSW Office of Environment and Heritage)</dcterms:contributor>
      <skos:topConceptOf rdf:resource="http://104.244.76.201/Bionet-ANDS-test/schema"/>
      <skos:narrower rdf:resource="http://104.244.76.201/Bionet-ANDS-test/schema/d1e224a1900"/>
      <skos:narrower rdf:resource="http://104.244.76.201/Bionet-ANDS-test/schema/d1e229a1900"/>
      <skos:narrower rdf:resource="http://104.244.76.201/Bionet-ANDS-test/schema/d1e271a1900"/>
      <skos:narrower rdf:resource="http://104.244.76.201/Bionet-ANDS-test/schema/d1e276a1900"/>
      <skos:narrower rdf:resource="http://104.244.76.201/Bionet-ANDS-test/schema/d1e286a1900"/>
      <skos:narrower rdf:resource="http://104.244.76.201/Bionet-ANDS-test/schema/d1e296a1900"/>
      <skos:narrower rdf:resource="http://104.244.76.201/Bionet-ANDS-test/schema/d1e307a1900"/>
      <skos:narrower rdf:resource="http://104.244.76.201/Bionet-ANDS-test/schema/d1e312a1900"/>
      <skos:narrower rdf:resource="http://104.244.76.201/Bionet-ANDS-test/schema/d1e317a1900"/>
      <skos:narrower rdf:resource="http://104.244.76.201/Bionet-ANDS-test/schema/d1e354a1900"/>
      <skos:narrower rdf:resource="http://104.244.76.201/Bionet-ANDS-test/schema/d1e365a1900"/>
      <skos:narrower rdf:resource="http://104.244.76.201/Bionet-ANDS-test/schema/d1e371a1900"/>
      <skos:narrower rdf:resource="http://104.244.76.201/Bionet-ANDS-test/schema/d1e379a1900"/>
      <skos:narrower rdf:resource="http://104.244.76.201/Bionet-ANDS-test/schema/d1e384a1900"/>
      <skos:narrower rdf:resource="http://104.244.76.201/Bionet-ANDS-test/schema/d1e394a1900"/>
      <skos:narrower rdf:resource="http://104.244.76.201/Bionet-ANDS-test/schema/d1e399a1900"/>
      <skos:narrower rdf:resource="http://104.244.76.201/Bionet-ANDS-test/schema/d1e404a1900"/>
      <skos:narrower rdf:resource="http://104.244.76.201/Bionet-ANDS-test/schema/d1e409a1900"/>
      <skos:narrower rdf:resource="http://104.244.76.201/Bionet-ANDS-test/schema/d1e440a1900"/>
      <skos:narrower rdf:resource="http://104.244.76.201/Bionet-ANDS-test/schema/d1e451a1900"/>
      <skos:narrower rdf:resource="http://104.244.76.201/Bionet-ANDS-test/schema/d1e481a1900"/>
   </rdf:Description>

   <rdf:Description rdf:about="http://104.244.76.201/Bionet-ANDS-test/schema/d1e494a1900">
      <rdf:type rdf:resource="http://www.w3.org/2004/02/skos/core#Concept"/>
      <skos:prefLabel xml:lang="en">Event</skos:prefLabel>
      <dcterms:creator>Bionet (NSW Office of Environment and Heritage)</dcterms:creator>
      <dcterms:contributor>Bionet (NSW Office of Environment and Heritage)</dcterms:contributor>
      <skos:topConceptOf rdf:resource="http://104.244.76.201/Bionet-ANDS-test/schema"/>
      <skos:narrower rdf:resource="http://104.244.76.201/Bionet-ANDS-test/schema/d1e495a1900"/>
      <skos:narrower rdf:resource="http://104.244.76.201/Bionet-ANDS-test/schema/d1e502a1900"/>
      <skos:narrower rdf:resource="http://104.244.76.201/Bionet-ANDS-test/schema/d1e507a1900"/>
      <skos:narrower rdf:resource="http://104.244.76.201/Bionet-ANDS-test/schema/d1e512a1900"/>
      <skos:narrower rdf:resource="http://104.244.76.201/Bionet-ANDS-test/schema/d1e519a1900"/>
      <skos:narrower rdf:resource="http://104.244.76.201/Bionet-ANDS-test/schema/d1e651a1900"/>
      <skos:narrower rdf:resource="http://104.244.76.201/Bionet-ANDS-test/schema/d1e656a1900"/>
   </rdf:Description>

   <rdf:Description rdf:about="http://104.244.76.201/Bionet-ANDS-test/schema/d1e661a1900">
      <rdf:type rdf:resource="http://www.w3.org/2004/02/skos/core#Concept"/>
      <skos:prefLabel xml:lang="en">Dcterms:Location</skos:prefLabel>
      <dcterms:creator>Bionet (NSW Office of Environment and Heritage)</dcterms:creator>
      <dcterms:contributor>Bionet (NSW Office of Environment and Heritage)</dcterms:contributor>
      <skos:topConceptOf rdf:resource="http://104.244.76.201/Bionet-ANDS-test/schema"/>
      <skos:narrower rdf:resource="http://104.244.76.201/Bionet-ANDS-test/schema/d1e662a1900"/>
      <skos:narrower rdf:resource="http://104.244.76.201/Bionet-ANDS-test/schema/d1e669a1900"/>
      <skos:narrower rdf:resource="http://104.244.76.201/Bionet-ANDS-test/schema/d1e676a1900"/>
      <skos:narrower rdf:resource="http://104.244.76.201/Bionet-ANDS-test/schema/d1e681a1900"/>
      <skos:narrower rdf:resource="http://104.244.76.201/Bionet-ANDS-test/schema/d1e686a1900"/>
      <skos:narrower rdf:resource="http://104.244.76.201/Bionet-ANDS-test/schema/d1e691a1900"/>
      <skos:narrower rdf:resource="http://104.244.76.201/Bionet-ANDS-test/schema/d1e696a1900"/>
      <skos:narrower rdf:resource="http://104.244.76.201/Bionet-ANDS-test/schema/d1e701a1900"/>
      <skos:narrower rdf:resource="http://104.244.76.201/Bionet-ANDS-test/schema/d1e706a1900"/>
      <skos:narrower rdf:resource="http://104.244.76.201/Bionet-ANDS-test/schema/d1e711a1900"/>
      <skos:narrower rdf:resource="http://104.244.76.201/Bionet-ANDS-test/schema/d1e718a1900"/>
      <skos:narrower rdf:resource="http://104.244.76.201/Bionet-ANDS-test/schema/d1e724a1900"/>
      <skos:narrower rdf:resource="http://104.244.76.201/Bionet-ANDS-test/schema/d1e729a1900"/>
      <skos:narrower rdf:resource="http://104.244.76.201/Bionet-ANDS-test/schema/d1e734a1900"/>
      <skos:narrower rdf:resource="http://104.244.76.201/Bionet-ANDS-test/schema/d1e739a1900"/>
      <skos:narrower rdf:resource="http://104.244.76.201/Bionet-ANDS-test/schema/d1e744a1900"/>
      <skos:narrower rdf:resource="http://104.244.76.201/Bionet-ANDS-test/schema/d1e749a1900"/>
      <skos:narrower rdf:resource="http://104.244.76.201/Bionet-ANDS-test/schema/d1e754a1900"/>
      <skos:narrower rdf:resource="http://104.244.76.201/Bionet-ANDS-test/schema/d1e759a1900"/>
   </rdf:Description>

   <rdf:Description rdf:about="http://104.244.76.201/Bionet-ANDS-test/schema/d1e764a1900">
      <rdf:type rdf:resource="http://www.w3.org/2004/02/skos/core#Concept"/>
      <skos:prefLabel xml:lang="en">Taxon</skos:prefLabel>
      <dcterms:creator>Bionet (NSW Office of Environment and Heritage)</dcterms:creator>
      <dcterms:contributor>Bionet (NSW Office of Environment and Heritage)</dcterms:contributor>
      <skos:topConceptOf rdf:resource="http://104.244.76.201/Bionet-ANDS-test/schema"/>
      <skos:narrower rdf:resource="http://104.244.76.201/Bionet-ANDS-test/schema/d1e765a1900"/>
      <skos:narrower rdf:resource="http://104.244.76.201/Bionet-ANDS-test/schema/d1e770a1900"/>
      <skos:narrower rdf:resource="http://104.244.76.201/Bionet-ANDS-test/schema/d1e775a1900"/>
      <skos:narrower rdf:resource="http://104.244.76.201/Bionet-ANDS-test/schema/d1e780a1900"/>
      <skos:narrower rdf:resource="http://104.244.76.201/Bionet-ANDS-test/schema/d1e785a1900"/>
      <skos:narrower rdf:resource="http://104.244.76.201/Bionet-ANDS-test/schema/d1e794a1900"/>
      <skos:narrower rdf:resource="http://104.244.76.201/Bionet-ANDS-test/schema/d1e799a1900"/>
      <skos:narrower rdf:resource="http://104.244.76.201/Bionet-ANDS-test/schema/d1e804a1900"/>
      <skos:narrower rdf:resource="http://104.244.76.201/Bionet-ANDS-test/schema/d1e809a1900"/>
      <skos:narrower rdf:resource="http://104.244.76.201/Bionet-ANDS-test/schema/d1e814a1900"/>
      <skos:narrower rdf:resource="http://104.244.76.201/Bionet-ANDS-test/schema/d1e819a1900"/>
      <skos:narrower rdf:resource="http://104.244.76.201/Bionet-ANDS-test/schema/d1e825a1900"/>
      <skos:narrower rdf:resource="http://104.244.76.201/Bionet-ANDS-test/schema/d1e830a1900"/>
      <skos:narrower rdf:resource="http://104.244.76.201/Bionet-ANDS-test/schema/d1e835a1900"/>
   </rdf:Description>

   <rdf:Description rdf:about="http://104.244.76.201/Bionet-ANDS-test/schema/d1e840a1900">
      <rdf:type rdf:resource="http://www.w3.org/2004/02/skos/core#Concept"/>
      <skos:prefLabel xml:lang="en">MeasurementOrFact</skos:prefLabel>
      <dcterms:creator>Bionet (NSW Office of Environment and Heritage)</dcterms:creator>
      <dcterms:contributor>Bionet (NSW Office of Environment and Heritage)</dcterms:contributor>
      <skos:topConceptOf rdf:resource="http://104.244.76.201/Bionet-ANDS-test/schema"/>
      <dcterms:description xml:lang="en">As discussed in the overview, additional measurements associated with a given sighting record will be supplied via a linked table using Darwin Core MeasurementOrFact. Each measurement will be linked back to the sighting record using the occurrenceID with the table below documenting the Darwin Core fields that will be made available via the species sighting web service.</dcterms:description>
      <skos:narrower rdf:resource="http://104.244.76.201/Bionet-ANDS-test/schema/d1e843a1900"/>
      <skos:narrower rdf:resource="http://104.244.76.201/Bionet-ANDS-test/schema/d1e850a1900"/>
      <skos:narrower rdf:resource="http://104.244.76.201/Bionet-ANDS-test/schema/d1e855a1900"/>
   </rdf:Description>

   <rdf:Description rdf:about="http://104.244.76.201/Bionet-ANDS-test/schema/d1e3a1900">
      <rdf:type rdf:resource="http://www.w3.org/2004/02/skos/core#Concept"/>
      <skos:prefLabel xml:lang="en">basisOfRecord</skos:prefLabel>
      <dcterms:creator>Bionet (NSW Office of Environment and Heritage)</dcterms:creator>
      <dcterms:contributor>Bionet (NSW Office of Environment and Heritage)</dcterms:contributor>
      <skos:broader rdf:resource="http://104.244.76.201/Bionet-ANDS-test/schema/d1e2a1900"/>
      <skos:definition xml:lang="en">The specific nature of the data record.</skos:definition>
      <skos:definition xml:lang="en">Based on the Darwin Core Type controlled vocabulary (http://rs.tdwg.org/dwc/terms/type-vocabulary/index.htm).</skos:definition>
      <skos:example xml:lang="en">"PreservedSpecimen", "FossilSpecimen", "LivingSpecimen", "HumanObservation", "MachineObservation".</skos:example>
   </rdf:Description>

   <rdf:Description rdf:about="http://104.244.76.201/Bionet-ANDS-test/schema/d1e10a1900">
      <rdf:type rdf:resource="http://www.w3.org/2004/02/skos/core#Concept"/>
      <skos:prefLabel xml:lang="en">collectionCode</skos:prefLabel>
      <dcterms:creator>Bionet (NSW Office of Environment and Heritage)</dcterms:creator>
      <dcterms:contributor>Bionet (NSW Office of Environment and Heritage)</dcterms:contributor>
      <skos:broader rdf:resource="http://104.244.76.201/Bionet-ANDS-test/schema/d1e2a1900"/>
      <skos:definition xml:lang="en">The name, acronym, coden, or initialism identifying the collection or data set from which the record was derived.</skos:definition>
      <skos:definition xml:lang="en">This will always be “BioNet Atlas of NSW Wildlife”</skos:definition>
      <skos:example xml:lang="en">“BioNet Atlas of NSW Wildlife”</skos:example>
   </rdf:Description>

   <rdf:Description rdf:about="http://104.244.76.201/Bionet-ANDS-test/schema/d1e17a1900">
      <rdf:type rdf:resource="http://www.w3.org/2004/02/skos/core#Concept"/>
      <skos:prefLabel xml:lang="en">dataGeneralizations</skos:prefLabel>
      <dcterms:creator>Bionet (NSW Office of Environment and Heritage)</dcterms:creator>
      <dcterms:contributor>Bionet (NSW Office of Environment and Heritage)</dcterms:contributor>
      <skos:broader rdf:resource="http://104.244.76.201/Bionet-ANDS-test/schema/d1e2a1900"/>
      <skos:definition xml:lang="en">Actions taken to make the shared data less specific or complete than in its original form.</skos:definition>
      <skos:definition xml:lang="en">In this case, when the record is for a species that is listed in the Sensitive Species data policy information will be given on the actual denaturing applied to the location data. It will be either:</skos:definition>
      <skos:definition xml:lang="en">coordinates rounded to 0.01°” for Category 3 species</skos:definition>
      <skos:definition xml:lang="en">oordinates rounded to 0.1°” for Category 2 species</skos:definition>
      <skos:definition xml:lang="en">The policy in full including the sensitive species listings can be located at:  http://www.environment.nsw.gov.au/policiesandguidelines/SensitiveSpeciesPolicy.htm</skos:definition>
      <skos:definition xml:lang="en">For Public and Licensed users the Observer Names will be provided as UserID, and there will be text =”The observer name has been changed to a unique User ID”</skos:definition>
      <skos:example xml:lang="en">“coordinates rounded to 0.01DEG” or “coordinates rounded to 0.1DEG”</skos:example>
      <skos:example xml:lang="en">“The observer name has been changed to a unique User ID”</skos:example>
   </rdf:Description>

   <rdf:Description rdf:about="http://104.244.76.201/Bionet-ANDS-test/schema/d1e34a1900">
      <rdf:type rdf:resource="http://www.w3.org/2004/02/skos/core#Concept"/>
      <skos:prefLabel xml:lang="en">datasetID</skos:prefLabel>
      <dcterms:creator>Bionet (NSW Office of Environment and Heritage)</dcterms:creator>
      <dcterms:contributor>Bionet (NSW Office of Environment and Heritage)</dcterms:contributor>
      <skos:broader rdf:resource="http://104.244.76.201/Bionet-ANDS-test/schema/d1e2a1900"/>
      <skos:definition xml:lang="en">An identifier for the set of data. May be a global unique identifier or an identifier specific to a collection or institution.</skos:definition>
      <skos:example xml:lang="en">12</skos:example>
   </rdf:Description>

   <rdf:Description rdf:about="http://104.244.76.201/Bionet-ANDS-test/schema/d1e39a1900">
      <rdf:type rdf:resource="http://www.w3.org/2004/02/skos/core#Concept"/>
      <skos:prefLabel xml:lang="en">datasetName</skos:prefLabel>
      <dcterms:creator>Bionet (NSW Office of Environment and Heritage)</dcterms:creator>
      <dcterms:contributor>Bionet (NSW Office of Environment and Heritage)</dcterms:contributor>
      <skos:broader rdf:resource="http://104.244.76.201/Bionet-ANDS-test/schema/d1e2a1900"/>
      <skos:definition xml:lang="en">The name identifying the data set from which the record was derived.</skos:definition>
      <skos:example xml:lang="en">“Atlas of Australian Birds 1”, “OEH Default Sightings”, “Grafton SF EIS Survey”</skos:example>
   </rdf:Description>

   <rdf:Description rdf:about="http://104.244.76.201/Bionet-ANDS-test/schema/d1e44a1900">
      <rdf:type rdf:resource="http://www.w3.org/2004/02/skos/core#Concept"/>
      <skos:prefLabel xml:lang="en">Dcterms_bibliographicCitation</skos:prefLabel>
      <dcterms:creator>Bionet (NSW Office of Environment and Heritage)</dcterms:creator>
      <dcterms:contributor>Bionet (NSW Office of Environment and Heritage)</dcterms:contributor>
      <skos:broader rdf:resource="http://104.244.76.201/Bionet-ANDS-test/schema/d1e2a1900"/>
      <skos:definition xml:lang="en">A bibliographic reference for the resource as a statement indicating how this record should be cited (attributed) when used.</skos:definition>
      <skos:definition xml:lang="en">This reference will be formatted as follows: “Atlas of NSW Wildlife &lt;current date&gt; &lt;HH:MM&gt; &lt;AM/PM&gt; + &lt;HH:MM offset from UTC&gt;”</skos:definition>
      <skos:definition xml:lang="en">Note: the date and time are AEST adjusted for daylight saving and reflect the data and time that the web service data was last refreshed from the source data (BioNet Atlas of NSW Wildlife database).</skos:definition>
      <skos:example xml:lang="en">“Atlas of NSW Wildlife 22/08/2014 12:47 AM + 10:00”</skos:example>
   </rdf:Description>

   <rdf:Description rdf:about="http://104.244.76.201/Bionet-ANDS-test/schema/d1e53a1900">
      <rdf:type rdf:resource="http://www.w3.org/2004/02/skos/core#Concept"/>
      <skos:prefLabel xml:lang="en">Dcterms_language</skos:prefLabel>
      <dcterms:creator>Bionet (NSW Office of Environment and Heritage)</dcterms:creator>
      <dcterms:contributor>Bionet (NSW Office of Environment and Heritage)</dcterms:contributor>
      <skos:broader rdf:resource="http://104.244.76.201/Bionet-ANDS-test/schema/d1e2a1900"/>
      <skos:definition xml:lang="en">The language of the resource based on RFC 4646 [RFC4646].</skos:definition>
      <skos:example xml:lang="en">"en" for English</skos:example>
   </rdf:Description>

   <rdf:Description rdf:about="http://104.244.76.201/Bionet-ANDS-test/schema/d1e58a1900">
      <rdf:type rdf:resource="http://www.w3.org/2004/02/skos/core#Concept"/>
      <skos:prefLabel xml:lang="en">Dcterms_modified</skos:prefLabel>
      <dcterms:creator>Bionet (NSW Office of Environment and Heritage)</dcterms:creator>
      <dcterms:contributor>Bionet (NSW Office of Environment and Heritage)</dcterms:contributor>
      <skos:broader rdf:resource="http://104.244.76.201/Bionet-ANDS-test/schema/d1e2a1900"/>
      <skos:definition xml:lang="en">The most recent date-time on which the resource was changed based on ISO 8601:2004(E).</skos:definition>
      <skos:definition xml:lang="en">Note:  OData only supports datetimeoffset, which mandates that the offset from UTC is given.  For many historical records in the BioNet Atlas of NSW Wildlife we cannot be certain that the server capturing the data at the time was adjusted for daylight savings.  To this end, the offset should not be relied upon.</skos:definition>
      <skos:example xml:lang="en">“15/03/2011 4:42 PM +11:00”2007 1pm UTC and 11 May 2008 3:30pm UTC, "2007-11-13/15" is the interval between 13 Nov 2007 and 15 Nov 2007.</skos:example>
   </rdf:Description>

   <rdf:Description rdf:about="http://104.244.76.201/Bionet-ANDS-test/schema/d1e65a1900">
      <rdf:type rdf:resource="http://www.w3.org/2004/02/skos/core#Concept"/>
      <skos:prefLabel xml:lang="en">Dcterms_rights</skos:prefLabel>
      <dcterms:creator>Bionet (NSW Office of Environment and Heritage)</dcterms:creator>
      <dcterms:contributor>Bionet (NSW Office of Environment and Heritage)</dcterms:contributor>
      <skos:broader rdf:resource="http://104.244.76.201/Bionet-ANDS-test/schema/d1e2a1900"/>
      <skos:definition xml:lang="en">Information about rights held in and over the resource. Typically, rights information includes a statement about various property rights associated with the resource, including intellectual property rights.</skos:definition>
      <skos:example xml:lang="en">"Creative Commons By Attribution"</skos:example>
   </rdf:Description>

   <rdf:Description rdf:about="http://104.244.76.201/Bionet-ANDS-test/schema/d1e70a1900">
      <rdf:type rdf:resource="http://www.w3.org/2004/02/skos/core#Concept"/>
      <skos:prefLabel xml:lang="en">Dcterms_rightsHolder</skos:prefLabel>
      <dcterms:creator>Bionet (NSW Office of Environment and Heritage)</dcterms:creator>
      <dcterms:contributor>Bionet (NSW Office of Environment and Heritage)</dcterms:contributor>
      <skos:broader rdf:resource="http://104.244.76.201/Bionet-ANDS-test/schema/d1e2a1900"/>
      <skos:definition xml:lang="en">A person or organization owning or managing rights over the resource.</skos:definition>
      <skos:example xml:lang="en">"Office of Environment and Heritage”, “Birds Australia”, “Australian Museum”</skos:example>
   </rdf:Description>

   <rdf:Description rdf:about="http://104.244.76.201/Bionet-ANDS-test/schema/d1e75a1900">
      <rdf:type rdf:resource="http://www.w3.org/2004/02/skos/core#Concept"/>
      <skos:prefLabel xml:lang="en">Dcterms_type</skos:prefLabel>
      <dcterms:creator>Bionet (NSW Office of Environment and Heritage)</dcterms:creator>
      <dcterms:contributor>Bionet (NSW Office of Environment and Heritage)</dcterms:contributor>
      <skos:broader rdf:resource="http://104.244.76.201/Bionet-ANDS-test/schema/d1e2a1900"/>
      <skos:definition xml:lang="en">The nature or genre of the resource. For Darwin Core, recommended best practice is to use the name of the class that defines the root of the record.</skos:definition>
      <skos:example xml:lang="en">"StillImage", "MovingImage", "Sound", "PhysicalObject", "Event".</skos:example>
   </rdf:Description>

   <rdf:Description rdf:about="http://104.244.76.201/Bionet-ANDS-test/schema/d1e81a1900">
      <rdf:type rdf:resource="http://www.w3.org/2004/02/skos/core#Concept"/>
      <skos:prefLabel xml:lang="en">dynamicProperties</skos:prefLabel>
      <dcterms:creator>Bionet (NSW Office of Environment and Heritage)</dcterms:creator>
      <dcterms:contributor>Bionet (NSW Office of Environment and Heritage)</dcterms:contributor>
      <skos:broader rdf:resource="http://104.244.76.201/Bionet-ANDS-test/schema/d1e2a1900"/>
      <dcterms:description xml:lang="en">The following table provides the full definitions of the data which will be passed using the dynamicProperties field in the Record-level terms table above.</dcterms:description>
      <skos:narrower rdf:resource="http://104.244.76.201/Bionet-ANDS-test/schema/d1e106a1900"/>
      <skos:narrower rdf:resource="http://104.244.76.201/Bionet-ANDS-test/schema/d1e111a1900"/>
      <skos:narrower rdf:resource="http://104.244.76.201/Bionet-ANDS-test/schema/d1e130a1900"/>
      <skos:narrower rdf:resource="http://104.244.76.201/Bionet-ANDS-test/schema/d1e135a1900"/>
      <skos:narrower rdf:resource="http://104.244.76.201/Bionet-ANDS-test/schema/d1e140a1900"/>
      <skos:narrower rdf:resource="http://104.244.76.201/Bionet-ANDS-test/schema/d1e147a1900"/>
      <skos:narrower rdf:resource="http://104.244.76.201/Bionet-ANDS-test/schema/d1e158a1900"/>
      <skos:narrower rdf:resource="http://104.244.76.201/Bionet-ANDS-test/schema/d1e165a1900"/>
      <skos:narrower rdf:resource="http://104.244.76.201/Bionet-ANDS-test/schema/d1e170a1900"/>
      <skos:narrower rdf:resource="http://104.244.76.201/Bionet-ANDS-test/schema/d1e180a1900"/>
      <skos:narrower rdf:resource="http://104.244.76.201/Bionet-ANDS-test/schema/d1e186a1900"/>
      <skos:narrower rdf:resource="http://104.244.76.201/Bionet-ANDS-test/schema/d1e201a1900"/>
      <skos:narrower rdf:resource="http://104.244.76.201/Bionet-ANDS-test/schema/d1e206a1900"/>
      <skos:narrower rdf:resource="http://104.244.76.201/Bionet-ANDS-test/schema/d1e211a1900"/>
      <skos:definition xml:lang="en">A list (concatenated and separated) of additional measurements, facts, characteristics, or assertions about the record. Meant to provide a mechanism for structured content such as key-value pairs.</skos:definition>
      <skos:definition xml:lang="en">See the dynamicProperties table below for the full definitions of additional data supplied via this field</skos:definition>
      <skos:example xml:lang="en">“BFMCS=8; GeogExtent=HR; MechanicalHRDescription= No slashing, trittering or tree removal; PotentialImpact=Exclude Bush Fire; ProfileID=10546; SpeciesFireDescritpion=No fire; Vulnerability=VH”</skos:example>
   </rdf:Description>

   <rdf:Description rdf:about="http://104.244.76.201/Bionet-ANDS-test/schema/d1e88a1900">
      <rdf:type rdf:resource="http://www.w3.org/2004/02/skos/core#Concept"/>
      <skos:prefLabel xml:lang="en">informationWithheld</skos:prefLabel>
      <dcterms:creator>Bionet (NSW Office of Environment and Heritage)</dcterms:creator>
      <dcterms:contributor>Bionet (NSW Office of Environment and Heritage)</dcterms:contributor>
      <skos:broader rdf:resource="http://104.244.76.201/Bionet-ANDS-test/schema/d1e2a1900"/>
      <skos:definition xml:lang="en">Additional information that exists, but that has not been shared in the given record.</skos:definition>
      <skos:example xml:lang="en">“The following fields have been withheld and are only available to licensed or OEH staff: locality, locationRemarks, occurenceRemarks, recordedBy”</skos:example>
   </rdf:Description>

   <rdf:Description rdf:about="http://104.244.76.201/Bionet-ANDS-test/schema/d1e93a1900">
      <rdf:type rdf:resource="http://www.w3.org/2004/02/skos/core#Concept"/>
      <skos:prefLabel xml:lang="en">institutionCode</skos:prefLabel>
      <dcterms:creator>Bionet (NSW Office of Environment and Heritage)</dcterms:creator>
      <dcterms:contributor>Bionet (NSW Office of Environment and Heritage)</dcterms:contributor>
      <skos:broader rdf:resource="http://104.244.76.201/Bionet-ANDS-test/schema/d1e2a1900"/>
      <skos:definition xml:lang="en">The name (or acronym) in use by the institution having custody of the object(s) or information referred to in the record.</skos:definition>
      <skos:example xml:lang="en">“NSW Office of Environment and Heritage”</skos:example>
   </rdf:Description>

   <rdf:Description rdf:about="http://104.244.76.201/Bionet-ANDS-test/schema/d1e98a1900">
      <rdf:type rdf:resource="http://www.w3.org/2004/02/skos/core#Concept"/>
      <skos:prefLabel xml:lang="en">ownerInstitutionCode</skos:prefLabel>
      <dcterms:creator>Bionet (NSW Office of Environment and Heritage)</dcterms:creator>
      <dcterms:contributor>Bionet (NSW Office of Environment and Heritage)</dcterms:contributor>
      <skos:broader rdf:resource="http://104.244.76.201/Bionet-ANDS-test/schema/d1e2a1900"/>
      <skos:definition xml:lang="en">The name (or acronym) in use by the institution having ownership of the object(s) or information referred to in the record.</skos:definition>
      <skos:example xml:lang="en">"Office of Environment and Heritage”, “Birds Australia”, “Australian Museum”</skos:example>
   </rdf:Description>

   <rdf:Description rdf:about="http://104.244.76.201/Bionet-ANDS-test/schema/d1e224a1900">
      <rdf:type rdf:resource="http://www.w3.org/2004/02/skos/core#Concept"/>
      <skos:prefLabel xml:lang="en">associatedReferences</skos:prefLabel>
      <dcterms:creator>Bionet (NSW Office of Environment and Heritage)</dcterms:creator>
      <dcterms:contributor>Bionet (NSW Office of Environment and Heritage)</dcterms:contributor>
      <skos:broader rdf:resource="http://104.244.76.201/Bionet-ANDS-test/schema/d1e223a1900"/>
      <skos:definition xml:lang="en">A list (concatenated and separated) of identifiers (publication, bibliographic reference, global unique identifier, URI) of literature associated with the Occurrence.</skos:definition>
      <skos:example xml:lang="en">"Christopher J. Conroy, Jennifer L. Neuwald. 2008. Phylogeographic study of the California vole, Microtus californicus Journal of Mammalogy, 89(3):755-767.".</skos:example>
   </rdf:Description>

   <rdf:Description rdf:about="http://104.244.76.201/Bionet-ANDS-test/schema/d1e229a1900">
      <rdf:type rdf:resource="http://www.w3.org/2004/02/skos/core#Concept"/>
      <skos:prefLabel xml:lang="en">austConservation</skos:prefLabel>
      <dcterms:creator>Bionet (NSW Office of Environment and Heritage)</dcterms:creator>
      <dcterms:contributor>Bionet (NSW Office of Environment and Heritage)</dcterms:contributor>
      <skos:broader rdf:resource="http://104.244.76.201/Bionet-ANDS-test/schema/d1e223a1900"/>
      <skos:narrowMatch rdf:resource="http://104.244.76.201/Bionet-ANDS-test/vocab/austConservation/d1e235a1900"/>
      <skos:narrowMatch rdf:resource="http://104.244.76.201/Bionet-ANDS-test/vocab/austConservation/d1e240a1900"/>
      <skos:narrowMatch rdf:resource="http://104.244.76.201/Bionet-ANDS-test/vocab/austConservation/d1e243a1900"/>
      <skos:narrowMatch rdf:resource="http://104.244.76.201/Bionet-ANDS-test/vocab/austConservation/d1e246a1900"/>
      <skos:narrowMatch rdf:resource="http://104.244.76.201/Bionet-ANDS-test/vocab/austConservation/d1e249a1900"/>
      <skos:narrowMatch rdf:resource="http://104.244.76.201/Bionet-ANDS-test/vocab/austConservation/d1e254a1900"/>
      <skos:narrowMatch rdf:resource="http://104.244.76.201/Bionet-ANDS-test/vocab/austConservation/d1e259a1900"/>
      <skos:narrowMatch rdf:resource="http://104.244.76.201/Bionet-ANDS-test/vocab/austConservation/d1e262a1900"/>
      <skos:narrowMatch rdf:resource="http://104.244.76.201/Bionet-ANDS-test/vocab/austConservation/d1e265a1900"/>
      <skos:narrowMatch rdf:resource="http://104.244.76.201/Bionet-ANDS-test/vocab/austConservation/d1e268a1900"/>
      <skos:definition xml:lang="en">The Legal Status of the species under the Commonwealth Environment Protection and Biodiversity Conservation Act 1999 (the EPBC Act), and Migratory Bird agreements (JAMBA, CAMBA and ROKAMBA). It uses the following controlled vocabulary:</skos:definition>
      <skos:example xml:lang="en">“CAMBA”</skos:example>
   </rdf:Description>

   <rdf:Description rdf:about="http://104.244.76.201/Bionet-ANDS-test/schema/d1e271a1900">
      <rdf:type rdf:resource="http://www.w3.org/2004/02/skos/core#Concept"/>
      <skos:prefLabel xml:lang="en">catalogNumber</skos:prefLabel>
      <dcterms:creator>Bionet (NSW Office of Environment and Heritage)</dcterms:creator>
      <dcterms:contributor>Bionet (NSW Office of Environment and Heritage)</dcterms:contributor>
      <skos:broader rdf:resource="http://104.244.76.201/Bionet-ANDS-test/schema/d1e223a1900"/>
      <skos:definition xml:lang="en">An identifier (preferably unique) for the record within the data set or collection.</skos:definition>
      <skos:example xml:lang="en">“WD9884”</skos:example>
   </rdf:Description>

   <rdf:Description rdf:about="http://104.244.76.201/Bionet-ANDS-test/schema/d1e276a1900">
      <rdf:type rdf:resource="http://www.w3.org/2004/02/skos/core#Concept"/>
      <skos:prefLabel xml:lang="en">consequence</skos:prefLabel>
      <dcterms:creator>Bionet (NSW Office of Environment and Heritage)</dcterms:creator>
      <dcterms:contributor>Bionet (NSW Office of Environment and Heritage)</dcterms:contributor>
      <skos:broader rdf:resource="http://104.244.76.201/Bionet-ANDS-test/schema/d1e223a1900"/>
      <skos:narrowMatch rdf:resource="http://104.244.76.201/Bionet-ANDS-test/vocab/consequence/d1e282a1900"/>
      <skos:narrowMatch rdf:resource="http://104.244.76.201/Bionet-ANDS-test/vocab/consequence/d1e283a1900"/>
      <skos:narrowMatch rdf:resource="http://104.244.76.201/Bionet-ANDS-test/vocab/consequence/d1e284a1900"/>
      <skos:narrowMatch rdf:resource="http://104.244.76.201/Bionet-ANDS-test/vocab/consequence/d1e285a1900"/>
      <skos:definition xml:lang="en">Final assessment as to the impact of Hazard Reduction activities on a species, based on the following controlled vocabulary:</skos:definition>
      <skos:example xml:lang="en">“Ma”</skos:example>
   </rdf:Description>

   <rdf:Description rdf:about="http://104.244.76.201/Bionet-ANDS-test/schema/d1e286a1900">
      <rdf:type rdf:resource="http://www.w3.org/2004/02/skos/core#Concept"/>
      <skos:prefLabel xml:lang="en">establishmentMeans</skos:prefLabel>
      <dcterms:creator>Bionet (NSW Office of Environment and Heritage)</dcterms:creator>
      <dcterms:contributor>Bionet (NSW Office of Environment and Heritage)</dcterms:contributor>
      <skos:broader rdf:resource="http://104.244.76.201/Bionet-ANDS-test/schema/d1e223a1900"/>
      <skos:narrowMatch rdf:resource="http://104.244.76.201/Bionet-ANDS-test/vocab/establishmentMeans/d1e292a1900"/>
      <skos:narrowMatch rdf:resource="http://104.244.76.201/Bionet-ANDS-test/vocab/establishmentMeans/d1e293a1900"/>
      <skos:narrowMatch rdf:resource="http://104.244.76.201/Bionet-ANDS-test/vocab/establishmentMeans/d1e294a1900"/>
      <skos:narrowMatch rdf:resource="http://104.244.76.201/Bionet-ANDS-test/vocab/establishmentMeans/d1e295a1900"/>
      <skos:definition xml:lang="en">The process by which the biological individual(s) represented in the Occurrence became established at the location. Based on the following controlled vocabulary:</skos:definition>
      <skos:example xml:lang="en">“Introduced”</skos:example>
   </rdf:Description>

   <rdf:Description rdf:about="http://104.244.76.201/Bionet-ANDS-test/schema/d1e296a1900">
      <rdf:type rdf:resource="http://www.w3.org/2004/02/skos/core#Concept"/>
      <skos:prefLabel xml:lang="en">estimateTypeCode</skos:prefLabel>
      <dcterms:creator>Bionet (NSW Office of Environment and Heritage)</dcterms:creator>
      <dcterms:contributor>Bionet (NSW Office of Environment and Heritage)</dcterms:contributor>
      <skos:broader rdf:resource="http://104.244.76.201/Bionet-ANDS-test/schema/d1e223a1900"/>
      <skos:narrowMatch rdf:resource="http://104.244.76.201/Bionet-ANDS-test/vocab/estimateTypeCode/d1e302a1900"/>
      <skos:narrowMatch rdf:resource="http://104.244.76.201/Bionet-ANDS-test/vocab/estimateTypeCode/d1e303a1900"/>
      <skos:narrowMatch rdf:resource="http://104.244.76.201/Bionet-ANDS-test/vocab/estimateTypeCode/d1e304a1900"/>
      <skos:narrowMatch rdf:resource="http://104.244.76.201/Bionet-ANDS-test/vocab/estimateTypeCode/d1e305a1900"/>
      <skos:narrowMatch rdf:resource="http://104.244.76.201/Bionet-ANDS-test/vocab/estimateTypeCode/d1e306a1900"/>
      <skos:definition xml:lang="en">Refers to the accuracy of the NumberIndividuals field using the following controlled vocabulary:</skos:definition>
      <skos:example xml:lang="en">“At least”</skos:example>
   </rdf:Description>

   <rdf:Description rdf:about="http://104.244.76.201/Bionet-ANDS-test/schema/d1e307a1900">
      <rdf:type rdf:resource="http://www.w3.org/2004/02/skos/core#Concept"/>
      <skos:prefLabel xml:lang="en">individualCount</skos:prefLabel>
      <dcterms:creator>Bionet (NSW Office of Environment and Heritage)</dcterms:creator>
      <dcterms:contributor>Bionet (NSW Office of Environment and Heritage)</dcterms:contributor>
      <skos:broader rdf:resource="http://104.244.76.201/Bionet-ANDS-test/schema/d1e223a1900"/>
      <skos:definition xml:lang="en">The number of individuals represented present at the time of the Occurrence.</skos:definition>
      <skos:example xml:lang="en">"25"</skos:example>
   </rdf:Description>

   <rdf:Description rdf:about="http://104.244.76.201/Bionet-ANDS-test/schema/d1e312a1900">
      <rdf:type rdf:resource="http://www.w3.org/2004/02/skos/core#Concept"/>
      <skos:prefLabel xml:lang="en">individualID</skos:prefLabel>
      <dcterms:creator>Bionet (NSW Office of Environment and Heritage)</dcterms:creator>
      <dcterms:contributor>Bionet (NSW Office of Environment and Heritage)</dcterms:contributor>
      <skos:broader rdf:resource="http://104.244.76.201/Bionet-ANDS-test/schema/d1e223a1900"/>
      <skos:definition xml:lang="en">An identifier for an individual or named group of individual organisms represented in the Occurrence. Meant to accommodate resampling of the same individual or group for monitoring purposes. May be a global unique identifier or an identifier specific to a data set.</skos:definition>
      <skos:example xml:lang="en">“DJS019”</skos:example>
   </rdf:Description>

   <rdf:Description rdf:about="http://104.244.76.201/Bionet-ANDS-test/schema/d1e317a1900">
      <rdf:type rdf:resource="http://www.w3.org/2004/02/skos/core#Concept"/>
      <skos:prefLabel xml:lang="en">observationType</skos:prefLabel>
      <dcterms:creator>Bionet (NSW Office of Environment and Heritage)</dcterms:creator>
      <dcterms:contributor>Bionet (NSW Office of Environment and Heritage)</dcterms:contributor>
      <skos:broader rdf:resource="http://104.244.76.201/Bionet-ANDS-test/schema/d1e223a1900"/>
      <skos:narrowMatch rdf:resource="http://104.244.76.201/Bionet-ANDS-test/vocab/observationType/d1e323a1900"/>
      <skos:narrowMatch rdf:resource="http://104.244.76.201/Bionet-ANDS-test/vocab/observationType/d1e324a1900"/>
      <skos:narrowMatch rdf:resource="http://104.244.76.201/Bionet-ANDS-test/vocab/observationType/d1e325a1900"/>
      <skos:narrowMatch rdf:resource="http://104.244.76.201/Bionet-ANDS-test/vocab/observationType/d1e326a1900"/>
      <skos:narrowMatch rdf:resource="http://104.244.76.201/Bionet-ANDS-test/vocab/observationType/d1e327a1900"/>
      <skos:narrowMatch rdf:resource="http://104.244.76.201/Bionet-ANDS-test/vocab/observationType/d1e328a1900"/>
      <skos:narrowMatch rdf:resource="http://104.244.76.201/Bionet-ANDS-test/vocab/observationType/d1e329a1900"/>
      <skos:narrowMatch rdf:resource="http://104.244.76.201/Bionet-ANDS-test/vocab/observationType/d1e330a1900"/>
      <skos:narrowMatch rdf:resource="http://104.244.76.201/Bionet-ANDS-test/vocab/observationType/d1e331a1900"/>
      <skos:narrowMatch rdf:resource="http://104.244.76.201/Bionet-ANDS-test/vocab/observationType/d1e332a1900"/>
      <skos:narrowMatch rdf:resource="http://104.244.76.201/Bionet-ANDS-test/vocab/observationType/d1e333a1900"/>
      <skos:narrowMatch rdf:resource="http://104.244.76.201/Bionet-ANDS-test/vocab/observationType/d1e335a1900"/>
      <skos:narrowMatch rdf:resource="http://104.244.76.201/Bionet-ANDS-test/vocab/observationType/d1e336a1900"/>
      <skos:narrowMatch rdf:resource="http://104.244.76.201/Bionet-ANDS-test/vocab/observationType/d1e337a1900"/>
      <skos:narrowMatch rdf:resource="http://104.244.76.201/Bionet-ANDS-test/vocab/observationType/d1e338a1900"/>
      <skos:narrowMatch rdf:resource="http://104.244.76.201/Bionet-ANDS-test/vocab/observationType/d1e339a1900"/>
      <skos:narrowMatch rdf:resource="http://104.244.76.201/Bionet-ANDS-test/vocab/observationType/d1e340a1900"/>
      <skos:narrowMatch rdf:resource="http://104.244.76.201/Bionet-ANDS-test/vocab/observationType/d1e341a1900"/>
      <skos:narrowMatch rdf:resource="http://104.244.76.201/Bionet-ANDS-test/vocab/observationType/d1e342a1900"/>
      <skos:narrowMatch rdf:resource="http://104.244.76.201/Bionet-ANDS-test/vocab/observationType/d1e343a1900"/>
      <skos:narrowMatch rdf:resource="http://104.244.76.201/Bionet-ANDS-test/vocab/observationType/d1e344a1900"/>
      <skos:narrowMatch rdf:resource="http://104.244.76.201/Bionet-ANDS-test/vocab/observationType/d1e345a1900"/>
      <skos:narrowMatch rdf:resource="http://104.244.76.201/Bionet-ANDS-test/vocab/observationType/d1e347a1900"/>
      <skos:narrowMatch rdf:resource="http://104.244.76.201/Bionet-ANDS-test/vocab/observationType/d1e348a1900"/>
      <skos:narrowMatch rdf:resource="http://104.244.76.201/Bionet-ANDS-test/vocab/observationType/d1e349a1900"/>
      <skos:narrowMatch rdf:resource="http://104.244.76.201/Bionet-ANDS-test/vocab/observationType/d1e350a1900"/>
      <skos:narrowMatch rdf:resource="http://104.244.76.201/Bionet-ANDS-test/vocab/observationType/d1e351a1900"/>
      <skos:narrowMatch rdf:resource="http://104.244.76.201/Bionet-ANDS-test/vocab/observationType/d1e352a1900"/>
      <skos:narrowMatch rdf:resource="http://104.244.76.201/Bionet-ANDS-test/vocab/observationType/d1e353a1900"/>
      <skos:definition xml:lang="en">Refers to the mode of observation. Uses a controlled vocabulary as follows:</skos:definition>
      <skos:example xml:lang="en">“Nest/Roost”</skos:example>
   </rdf:Description>

   <rdf:Description rdf:about="http://104.244.76.201/Bionet-ANDS-test/schema/d1e354a1900">
      <rdf:type rdf:resource="http://www.w3.org/2004/02/skos/core#Concept"/>
      <skos:prefLabel xml:lang="en">occurrenceID</skos:prefLabel>
      <dcterms:creator>Bionet (NSW Office of Environment and Heritage)</dcterms:creator>
      <dcterms:contributor>Bionet (NSW Office of Environment and Heritage)</dcterms:contributor>
      <skos:broader rdf:resource="http://104.244.76.201/Bionet-ANDS-test/schema/d1e223a1900"/>
      <skos:definition xml:lang="en">An identifier for the Occurrence (as opposed to a particular digital record of the occurrence).</skos:definition>
      <skos:definition xml:lang="en">In the absence of a persistent global unique identifier, construct one from a combination of identifiers in the record that will most closely make the occurrenceID globally unique.</skos:definition>
      <skos:definition xml:lang="en">For this service it will be constructed according to the recommended Darwin Core formula as follows:</skos:definition>
      <skos:definition xml:lang="en">"urn:catalog:[institutionCode]:[collectionCode]:[catalogNumber]</skos:definition>
      <skos:example xml:lang="en">"urn:catalog: NSW Office of Environment and Heritage: BioNet Atlas of NSW Wildlife: WD9884".</skos:example>
   </rdf:Description>

   <rdf:Description rdf:about="http://104.244.76.201/Bionet-ANDS-test/schema/d1e365a1900">
      <rdf:type rdf:resource="http://www.w3.org/2004/02/skos/core#Concept"/>
      <skos:prefLabel xml:lang="en">occurrenceRemarks</skos:prefLabel>
      <dcterms:creator>Bionet (NSW Office of Environment and Heritage)</dcterms:creator>
      <dcterms:contributor>Bionet (NSW Office of Environment and Heritage)</dcterms:contributor>
      <skos:broader rdf:resource="http://104.244.76.201/Bionet-ANDS-test/schema/d1e223a1900"/>
      <skos:definition xml:lang="en">Comments or notes about the Occurrence.</skos:definition>
      <skos:example xml:lang="en">"found dead on road".</skos:example>
   </rdf:Description>

   <rdf:Description rdf:about="http://104.244.76.201/Bionet-ANDS-test/schema/d1e371a1900">
      <rdf:type rdf:resource="http://www.w3.org/2004/02/skos/core#Concept"/>
      <skos:prefLabel xml:lang="en">occurrenceStatus</skos:prefLabel>
      <dcterms:creator>Bionet (NSW Office of Environment and Heritage)</dcterms:creator>
      <dcterms:contributor>Bionet (NSW Office of Environment and Heritage)</dcterms:contributor>
      <skos:broader rdf:resource="http://104.244.76.201/Bionet-ANDS-test/schema/d1e223a1900"/>
      <skos:narrowMatch rdf:resource="http://104.244.76.201/Bionet-ANDS-test/vocab/occurrenceStatus/d1e377a1900"/>
      <skos:narrowMatch rdf:resource="http://104.244.76.201/Bionet-ANDS-test/vocab/occurrenceStatus/d1e378a1900"/>
      <skos:definition xml:lang="en">A statement about the presence or absence of a Taxon at a Location. Based on the following controlled vocabulary:</skos:definition>
      <skos:example xml:lang="en">"Present”</skos:example>
   </rdf:Description>

   <rdf:Description rdf:about="http://104.244.76.201/Bionet-ANDS-test/schema/d1e379a1900">
      <rdf:type rdf:resource="http://www.w3.org/2004/02/skos/core#Concept"/>
      <skos:prefLabel xml:lang="en">otherCatalogNumbers</skos:prefLabel>
      <dcterms:creator>Bionet (NSW Office of Environment and Heritage)</dcterms:creator>
      <dcterms:contributor>Bionet (NSW Office of Environment and Heritage)</dcterms:contributor>
      <skos:broader rdf:resource="http://104.244.76.201/Bionet-ANDS-test/schema/d1e223a1900"/>
      <skos:definition xml:lang="en">A list (concatenated and separated) of previous or alternate fully qualified catalog numbers or other human-used identifiers for the same Occurrence, whether in the current or any other data set or collection.</skos:definition>
      <skos:example xml:lang="en">"The Australian Museum, Sydney R10694", "Royal Botanic Gardens &amp; National Herbarium of NSW, Sydney NSW227432".</skos:example>
   </rdf:Description>

   <rdf:Description rdf:about="http://104.244.76.201/Bionet-ANDS-test/schema/d1e384a1900">
      <rdf:type rdf:resource="http://www.w3.org/2004/02/skos/core#Concept"/>
      <skos:prefLabel xml:lang="en">PNFFilter</skos:prefLabel>
      <dcterms:creator>Bionet (NSW Office of Environment and Heritage)</dcterms:creator>
      <dcterms:contributor>Bionet (NSW Office of Environment and Heritage)</dcterms:contributor>
      <skos:broader rdf:resource="http://104.244.76.201/Bionet-ANDS-test/schema/d1e223a1900"/>
      <skos:narrowMatch rdf:resource="http://104.244.76.201/Bionet-ANDS-test/vocab/PNFFilter/d1e392a1900"/>
      <skos:narrowMatch rdf:resource="http://104.244.76.201/Bionet-ANDS-test/vocab/PNFFilter/d1e393a1900"/>
      <skos:definition xml:lang="en">Indicator as to whether the record is relevant to the Private Native Forestry Code of Practice based on the following controlled vocabulary:</skos:definition>
      <skos:definition xml:lang="en">See http://www.epa.nsw.gov.au/pnf/CodeofPractice.htm for more details and to download the code of practice.</skos:definition>
      <skos:example xml:lang="en">“Y”, “N”</skos:example>
   </rdf:Description>

   <rdf:Description rdf:about="http://104.244.76.201/Bionet-ANDS-test/schema/d1e394a1900">
      <rdf:type rdf:resource="http://www.w3.org/2004/02/skos/core#Concept"/>
      <skos:prefLabel xml:lang="en">populationName</skos:prefLabel>
      <dcterms:creator>Bionet (NSW Office of Environment and Heritage)</dcterms:creator>
      <dcterms:contributor>Bionet (NSW Office of Environment and Heritage)</dcterms:contributor>
      <skos:broader rdf:resource="http://104.244.76.201/Bionet-ANDS-test/schema/d1e223a1900"/>
      <skos:definition xml:lang="en">Where the observation relates to the occurrence of a species within an endangered population as listed under the Threatened Species conservation Act 1995, the name of the threatened population will be given here</skos:definition>
      <skos:example xml:lang="en">"Emu population in the New South Wales North Coast Bioregion and Port Stephens local government area"</skos:example>
   </rdf:Description>

   <rdf:Description rdf:about="http://104.244.76.201/Bionet-ANDS-test/schema/d1e399a1900">
      <rdf:type rdf:resource="http://www.w3.org/2004/02/skos/core#Concept"/>
      <skos:prefLabel xml:lang="en">recordedBy</skos:prefLabel>
      <dcterms:creator>Bionet (NSW Office of Environment and Heritage)</dcterms:creator>
      <dcterms:contributor>Bionet (NSW Office of Environment and Heritage)</dcterms:contributor>
      <skos:broader rdf:resource="http://104.244.76.201/Bionet-ANDS-test/schema/d1e223a1900"/>
      <skos:definition xml:lang="en">A list (concatenated and separated) of names of people, groups, or organizations responsible for recording the original Occurrence.</skos:definition>
      <skos:example xml:lang="en">"Oliver P. Pearson; Anita K. Pearson"</skos:example>
   </rdf:Description>

   <rdf:Description rdf:about="http://104.244.76.201/Bionet-ANDS-test/schema/d1e404a1900">
      <rdf:type rdf:resource="http://www.w3.org/2004/02/skos/core#Concept"/>
      <skos:prefLabel xml:lang="en">recordNumber</skos:prefLabel>
      <dcterms:creator>Bionet (NSW Office of Environment and Heritage)</dcterms:creator>
      <dcterms:contributor>Bionet (NSW Office of Environment and Heritage)</dcterms:contributor>
      <skos:broader rdf:resource="http://104.244.76.201/Bionet-ANDS-test/schema/d1e223a1900"/>
      <skos:definition xml:lang="en">An identifier given to the Occurrence at the time it was recorded. Often serves as a link between field notes and an Occurrence record, such as a specimen collector's number.</skos:definition>
      <skos:example xml:lang="en">"OPP 7101"</skos:example>
   </rdf:Description>

   <rdf:Description rdf:about="http://104.244.76.201/Bionet-ANDS-test/schema/d1e409a1900">
      <rdf:type rdf:resource="http://www.w3.org/2004/02/skos/core#Concept"/>
      <skos:prefLabel xml:lang="en">reproductiveCondition</skos:prefLabel>
      <dcterms:creator>Bionet (NSW Office of Environment and Heritage)</dcterms:creator>
      <dcterms:contributor>Bionet (NSW Office of Environment and Heritage)</dcterms:contributor>
      <skos:broader rdf:resource="http://104.244.76.201/Bionet-ANDS-test/schema/d1e223a1900"/>
      <skos:narrower rdf:resource="http://104.244.76.201/Bionet-ANDS-test/schema/d1e414a1900"/>
      <skos:narrower rdf:resource="http://104.244.76.201/Bionet-ANDS-test/schema/d1e424a1900"/>
      <skos:definition xml:lang="en">The reproductive condition of the biological individual(s) represented in the Occurrence.</skos:definition>
      <skos:example xml:lang="en">“- Not breeding,A Adult,D Distraction display,E Eggs,I Immature (subadult),M Nestling,N Nesting”</skos:example>
   </rdf:Description>

   <rdf:Description rdf:about="http://104.244.76.201/Bionet-ANDS-test/schema/d1e440a1900">
      <rdf:type rdf:resource="http://www.w3.org/2004/02/skos/core#Concept"/>
      <skos:prefLabel xml:lang="en">sex</skos:prefLabel>
      <dcterms:creator>Bionet (NSW Office of Environment and Heritage)</dcterms:creator>
      <dcterms:contributor>Bionet (NSW Office of Environment and Heritage)</dcterms:contributor>
      <skos:broader rdf:resource="http://104.244.76.201/Bionet-ANDS-test/schema/d1e223a1900"/>
      <skos:narrowMatch rdf:resource="http://104.244.76.201/Bionet-ANDS-test/vocab/sex/d1e446a1900"/>
      <skos:narrowMatch rdf:resource="http://104.244.76.201/Bionet-ANDS-test/vocab/sex/d1e447a1900"/>
      <skos:narrowMatch rdf:resource="http://104.244.76.201/Bionet-ANDS-test/vocab/sex/d1e448a1900"/>
      <skos:narrowMatch rdf:resource="http://104.244.76.201/Bionet-ANDS-test/vocab/sex/d1e449a1900"/>
      <skos:narrowMatch rdf:resource="http://104.244.76.201/Bionet-ANDS-test/vocab/sex/d1e450a1900"/>
      <skos:definition xml:lang="en">The sex of the biological individual(s) represented in the Occurrence based on the following controlled vocabulary:</skos:definition>
      <skos:example xml:lang="en">"Female”, “Unknown”</skos:example>
   </rdf:Description>

   <rdf:Description rdf:about="http://104.244.76.201/Bionet-ANDS-test/schema/d1e451a1900">
      <rdf:type rdf:resource="http://www.w3.org/2004/02/skos/core#Concept"/>
      <skos:prefLabel xml:lang="en">stateConservation</skos:prefLabel>
      <dcterms:creator>Bionet (NSW Office of Environment and Heritage)</dcterms:creator>
      <dcterms:contributor>Bionet (NSW Office of Environment and Heritage)</dcterms:contributor>
      <skos:broader rdf:resource="http://104.244.76.201/Bionet-ANDS-test/schema/d1e223a1900"/>
      <skos:narrowMatch rdf:resource="http://104.244.76.201/Bionet-ANDS-test/vocab/stateConservation/d1e457a1900"/>
      <skos:narrowMatch rdf:resource="http://104.244.76.201/Bionet-ANDS-test/vocab/stateConservation/d1e460a1900"/>
      <skos:narrowMatch rdf:resource="http://104.244.76.201/Bionet-ANDS-test/vocab/stateConservation/d1e463a1900"/>
      <skos:narrowMatch rdf:resource="http://104.244.76.201/Bionet-ANDS-test/vocab/stateConservation/d1e466a1900"/>
      <skos:narrowMatch rdf:resource="http://104.244.76.201/Bionet-ANDS-test/vocab/stateConservation/d1e469a1900"/>
      <skos:narrowMatch rdf:resource="http://104.244.76.201/Bionet-ANDS-test/vocab/stateConservation/d1e472a1900"/>
      <skos:narrowMatch rdf:resource="http://104.244.76.201/Bionet-ANDS-test/vocab/stateConservation/d1e475a1900"/>
      <skos:narrowMatch rdf:resource="http://104.244.76.201/Bionet-ANDS-test/vocab/stateConservation/d1e478a1900"/>
      <skos:definition xml:lang="en">The Legal Status of the species within NSW under the Threatened Species Conservation Act (TSC Act 1995), the National Parks and Wildlife Act 1974 (NPW Act 1974), the Fisheries Management Act 1994 No. 38 (FM Act 1994) and the Sensitive Species Data Policy (SSDP).</skos:definition>
      <skos:example xml:lang="en">“Protected”, “Endangered, Category 2 Sensitive Species”</skos:example>
   </rdf:Description>

   <rdf:Description rdf:about="http://104.244.76.201/Bionet-ANDS-test/schema/d1e481a1900">
      <rdf:type rdf:resource="http://www.w3.org/2004/02/skos/core#Concept"/>
      <skos:prefLabel xml:lang="en">status</skos:prefLabel>
      <dcterms:creator>Bionet (NSW Office of Environment and Heritage)</dcterms:creator>
      <dcterms:contributor>Bionet (NSW Office of Environment and Heritage)</dcterms:contributor>
      <skos:broader rdf:resource="http://104.244.76.201/Bionet-ANDS-test/schema/d1e223a1900"/>
      <skos:narrowMatch rdf:resource="http://104.244.76.201/Bionet-ANDS-test/vocab/status/d1e487a1900"/>
      <skos:narrowMatch rdf:resource="http://104.244.76.201/Bionet-ANDS-test/vocab/status/d1e488a1900"/>
      <skos:narrowMatch rdf:resource="http://104.244.76.201/Bionet-ANDS-test/vocab/status/d1e489a1900"/>
      <skos:narrowMatch rdf:resource="http://104.244.76.201/Bionet-ANDS-test/vocab/status/d1e490a1900"/>
      <skos:narrowMatch rdf:resource="http://104.244.76.201/Bionet-ANDS-test/vocab/status/d1e491a1900"/>
      <skos:narrowMatch rdf:resource="http://104.244.76.201/Bionet-ANDS-test/vocab/status/d1e492a1900"/>
      <skos:narrowMatch rdf:resource="http://104.244.76.201/Bionet-ANDS-test/vocab/status/d1e493a1900"/>
      <skos:definition xml:lang="en">The status of the record with respect to its validity as per the following controlled vocabulary:</skos:definition>
      <skos:example xml:lang="en">“Suspect”, “Rejected as certainly incorrect”</skos:example>
   </rdf:Description>

   <rdf:Description rdf:about="http://104.244.76.201/Bionet-ANDS-test/schema/d1e495a1900">
      <rdf:type rdf:resource="http://www.w3.org/2004/02/skos/core#Concept"/>
      <skos:prefLabel xml:lang="en">eventDate</skos:prefLabel>
      <dcterms:creator>Bionet (NSW Office of Environment and Heritage)</dcterms:creator>
      <dcterms:contributor>Bionet (NSW Office of Environment and Heritage)</dcterms:contributor>
      <skos:broader rdf:resource="http://104.244.76.201/Bionet-ANDS-test/schema/d1e494a1900"/>
      <skos:definition xml:lang="en">The date-time or interval during which an Event occurred. For occurrences, this is the date-time when the event was recorded.</skos:definition>
      <skos:definition xml:lang="en">As per recommended best practice encoded using ISO 8601:2004(E).</skos:definition>
      <skos:example xml:lang="en">“1978-06-01/1978-06-28”</skos:example>
   </rdf:Description>

   <rdf:Description rdf:about="http://104.244.76.201/Bionet-ANDS-test/schema/d1e502a1900">
      <rdf:type rdf:resource="http://www.w3.org/2004/02/skos/core#Concept"/>
      <skos:prefLabel xml:lang="en">eventID</skos:prefLabel>
      <dcterms:creator>Bionet (NSW Office of Environment and Heritage)</dcterms:creator>
      <dcterms:contributor>Bionet (NSW Office of Environment and Heritage)</dcterms:contributor>
      <skos:broader rdf:resource="http://104.244.76.201/Bionet-ANDS-test/schema/d1e494a1900"/>
      <skos:definition xml:lang="en">The unique key assigned to a Census. A Census is a time distinct assessment conducted within a survey at a designated site.</skos:definition>
      <skos:example xml:lang="en">“CPXEI0000001”</skos:example>
   </rdf:Description>

   <rdf:Description rdf:about="http://104.244.76.201/Bionet-ANDS-test/schema/d1e507a1900">
      <rdf:type rdf:resource="http://www.w3.org/2004/02/skos/core#Concept"/>
      <skos:prefLabel xml:lang="en">eventRemarks</skos:prefLabel>
      <dcterms:creator>Bionet (NSW Office of Environment and Heritage)</dcterms:creator>
      <dcterms:contributor>Bionet (NSW Office of Environment and Heritage)</dcterms:contributor>
      <skos:broader rdf:resource="http://104.244.76.201/Bionet-ANDS-test/schema/d1e494a1900"/>
      <skos:definition xml:lang="en">Comments or notes about the Event.</skos:definition>
      <skos:example xml:lang="en">"after the recent rains the river is nearly at flood stage".</skos:example>
   </rdf:Description>

   <rdf:Description rdf:about="http://104.244.76.201/Bionet-ANDS-test/schema/d1e512a1900">
      <rdf:type rdf:resource="http://www.w3.org/2004/02/skos/core#Concept"/>
      <skos:prefLabel xml:lang="en">eventTime</skos:prefLabel>
      <dcterms:creator>Bionet (NSW Office of Environment and Heritage)</dcterms:creator>
      <dcterms:contributor>Bionet (NSW Office of Environment and Heritage)</dcterms:contributor>
      <skos:broader rdf:resource="http://104.244.76.201/Bionet-ANDS-test/schema/d1e494a1900"/>
      <skos:definition xml:lang="en">The time or interval during which an Event occurred.</skos:definition>
      <skos:definition xml:lang="en">As per recommended best practice encoded using ISO 8601:2004(E).</skos:definition>
      <skos:example xml:lang="en">“10:00:00/10:05:00”</skos:example>
   </rdf:Description>

   <rdf:Description rdf:about="http://104.244.76.201/Bionet-ANDS-test/schema/d1e519a1900">
      <rdf:type rdf:resource="http://www.w3.org/2004/02/skos/core#Concept"/>
      <skos:prefLabel xml:lang="en">habitat</skos:prefLabel>
      <dcterms:creator>Bionet (NSW Office of Environment and Heritage)</dcterms:creator>
      <dcterms:contributor>Bionet (NSW Office of Environment and Heritage)</dcterms:contributor>
      <skos:broader rdf:resource="http://104.244.76.201/Bionet-ANDS-test/schema/d1e494a1900"/>
      <skos:narrowMatch rdf:resource="http://104.244.76.201/Bionet-ANDS-test/vocab/habitat/d1e525a1900"/>
      <skos:narrowMatch rdf:resource="http://104.244.76.201/Bionet-ANDS-test/vocab/habitat/d1e526a1900"/>
      <skos:narrowMatch rdf:resource="http://104.244.76.201/Bionet-ANDS-test/vocab/habitat/d1e527a1900"/>
      <skos:narrowMatch rdf:resource="http://104.244.76.201/Bionet-ANDS-test/vocab/habitat/d1e528a1900"/>
      <skos:narrowMatch rdf:resource="http://104.244.76.201/Bionet-ANDS-test/vocab/habitat/d1e529a1900"/>
      <skos:narrowMatch rdf:resource="http://104.244.76.201/Bionet-ANDS-test/vocab/habitat/d1e530a1900"/>
      <skos:narrowMatch rdf:resource="http://104.244.76.201/Bionet-ANDS-test/vocab/habitat/d1e531a1900"/>
      <skos:narrowMatch rdf:resource="http://104.244.76.201/Bionet-ANDS-test/vocab/habitat/d1e532a1900"/>
      <skos:narrowMatch rdf:resource="http://104.244.76.201/Bionet-ANDS-test/vocab/habitat/d1e533a1900"/>
      <skos:narrowMatch rdf:resource="http://104.244.76.201/Bionet-ANDS-test/vocab/habitat/d1e534a1900"/>
      <skos:narrowMatch rdf:resource="http://104.244.76.201/Bionet-ANDS-test/vocab/habitat/d1e535a1900"/>
      <skos:narrowMatch rdf:resource="http://104.244.76.201/Bionet-ANDS-test/vocab/habitat/d1e537a1900"/>
      <skos:narrowMatch rdf:resource="http://104.244.76.201/Bionet-ANDS-test/vocab/habitat/d1e538a1900"/>
      <skos:narrowMatch rdf:resource="http://104.244.76.201/Bionet-ANDS-test/vocab/habitat/d1e539a1900"/>
      <skos:narrowMatch rdf:resource="http://104.244.76.201/Bionet-ANDS-test/vocab/habitat/d1e540a1900"/>
      <skos:narrowMatch rdf:resource="http://104.244.76.201/Bionet-ANDS-test/vocab/habitat/d1e541a1900"/>
      <skos:narrowMatch rdf:resource="http://104.244.76.201/Bionet-ANDS-test/vocab/habitat/d1e542a1900"/>
      <skos:narrowMatch rdf:resource="http://104.244.76.201/Bionet-ANDS-test/vocab/habitat/d1e543a1900"/>
      <skos:narrowMatch rdf:resource="http://104.244.76.201/Bionet-ANDS-test/vocab/habitat/d1e544a1900"/>
      <skos:narrowMatch rdf:resource="http://104.244.76.201/Bionet-ANDS-test/vocab/habitat/d1e545a1900"/>
      <skos:narrowMatch rdf:resource="http://104.244.76.201/Bionet-ANDS-test/vocab/habitat/d1e546a1900"/>
      <skos:narrowMatch rdf:resource="http://104.244.76.201/Bionet-ANDS-test/vocab/habitat/d1e547a1900"/>
      <skos:narrowMatch rdf:resource="http://104.244.76.201/Bionet-ANDS-test/vocab/habitat/d1e549a1900"/>
      <skos:narrowMatch rdf:resource="http://104.244.76.201/Bionet-ANDS-test/vocab/habitat/d1e550a1900"/>
      <skos:narrowMatch rdf:resource="http://104.244.76.201/Bionet-ANDS-test/vocab/habitat/d1e551a1900"/>
      <skos:narrowMatch rdf:resource="http://104.244.76.201/Bionet-ANDS-test/vocab/habitat/d1e552a1900"/>
      <skos:narrowMatch rdf:resource="http://104.244.76.201/Bionet-ANDS-test/vocab/habitat/d1e553a1900"/>
      <skos:narrowMatch rdf:resource="http://104.244.76.201/Bionet-ANDS-test/vocab/habitat/d1e554a1900"/>
      <skos:narrowMatch rdf:resource="http://104.244.76.201/Bionet-ANDS-test/vocab/habitat/d1e555a1900"/>
      <skos:narrowMatch rdf:resource="http://104.244.76.201/Bionet-ANDS-test/vocab/habitat/d1e556a1900"/>
      <skos:narrowMatch rdf:resource="http://104.244.76.201/Bionet-ANDS-test/vocab/habitat/d1e557a1900"/>
      <skos:narrowMatch rdf:resource="http://104.244.76.201/Bionet-ANDS-test/vocab/habitat/d1e558a1900"/>
      <skos:narrowMatch rdf:resource="http://104.244.76.201/Bionet-ANDS-test/vocab/habitat/d1e559a1900"/>
      <skos:narrowMatch rdf:resource="http://104.244.76.201/Bionet-ANDS-test/vocab/habitat/d1e561a1900"/>
      <skos:narrowMatch rdf:resource="http://104.244.76.201/Bionet-ANDS-test/vocab/habitat/d1e562a1900"/>
      <skos:narrowMatch rdf:resource="http://104.244.76.201/Bionet-ANDS-test/vocab/habitat/d1e563a1900"/>
      <skos:narrowMatch rdf:resource="http://104.244.76.201/Bionet-ANDS-test/vocab/habitat/d1e564a1900"/>
      <skos:narrowMatch rdf:resource="http://104.244.76.201/Bionet-ANDS-test/vocab/habitat/d1e565a1900"/>
      <skos:narrowMatch rdf:resource="http://104.244.76.201/Bionet-ANDS-test/vocab/habitat/d1e566a1900"/>
      <skos:narrowMatch rdf:resource="http://104.244.76.201/Bionet-ANDS-test/vocab/habitat/d1e567a1900"/>
      <skos:narrowMatch rdf:resource="http://104.244.76.201/Bionet-ANDS-test/vocab/habitat/d1e568a1900"/>
      <skos:narrowMatch rdf:resource="http://104.244.76.201/Bionet-ANDS-test/vocab/habitat/d1e569a1900"/>
      <skos:narrowMatch rdf:resource="http://104.244.76.201/Bionet-ANDS-test/vocab/habitat/d1e570a1900"/>
      <skos:narrowMatch rdf:resource="http://104.244.76.201/Bionet-ANDS-test/vocab/habitat/d1e571a1900"/>
      <skos:narrowMatch rdf:resource="http://104.244.76.201/Bionet-ANDS-test/vocab/habitat/d1e573a1900"/>
      <skos:narrowMatch rdf:resource="http://104.244.76.201/Bionet-ANDS-test/vocab/habitat/d1e574a1900"/>
      <skos:narrowMatch rdf:resource="http://104.244.76.201/Bionet-ANDS-test/vocab/habitat/d1e575a1900"/>
      <skos:narrowMatch rdf:resource="http://104.244.76.201/Bionet-ANDS-test/vocab/habitat/d1e576a1900"/>
      <skos:narrowMatch rdf:resource="http://104.244.76.201/Bionet-ANDS-test/vocab/habitat/d1e577a1900"/>
      <skos:narrowMatch rdf:resource="http://104.244.76.201/Bionet-ANDS-test/vocab/habitat/d1e578a1900"/>
      <skos:narrowMatch rdf:resource="http://104.244.76.201/Bionet-ANDS-test/vocab/habitat/d1e579a1900"/>
      <skos:narrowMatch rdf:resource="http://104.244.76.201/Bionet-ANDS-test/vocab/habitat/d1e580a1900"/>
      <skos:narrowMatch rdf:resource="http://104.244.76.201/Bionet-ANDS-test/vocab/habitat/d1e581a1900"/>
      <skos:narrowMatch rdf:resource="http://104.244.76.201/Bionet-ANDS-test/vocab/habitat/d1e582a1900"/>
      <skos:narrowMatch rdf:resource="http://104.244.76.201/Bionet-ANDS-test/vocab/habitat/d1e583a1900"/>
      <skos:narrowMatch rdf:resource="http://104.244.76.201/Bionet-ANDS-test/vocab/habitat/d1e585a1900"/>
      <skos:narrowMatch rdf:resource="http://104.244.76.201/Bionet-ANDS-test/vocab/habitat/d1e586a1900"/>
      <skos:narrowMatch rdf:resource="http://104.244.76.201/Bionet-ANDS-test/vocab/habitat/d1e587a1900"/>
      <skos:narrowMatch rdf:resource="http://104.244.76.201/Bionet-ANDS-test/vocab/habitat/d1e588a1900"/>
      <skos:narrowMatch rdf:resource="http://104.244.76.201/Bionet-ANDS-test/vocab/habitat/d1e589a1900"/>
      <skos:narrowMatch rdf:resource="http://104.244.76.201/Bionet-ANDS-test/vocab/habitat/d1e590a1900"/>
      <skos:narrowMatch rdf:resource="http://104.244.76.201/Bionet-ANDS-test/vocab/habitat/d1e591a1900"/>
      <skos:narrowMatch rdf:resource="http://104.244.76.201/Bionet-ANDS-test/vocab/habitat/d1e592a1900"/>
      <skos:narrowMatch rdf:resource="http://104.244.76.201/Bionet-ANDS-test/vocab/habitat/d1e593a1900"/>
      <skos:narrowMatch rdf:resource="http://104.244.76.201/Bionet-ANDS-test/vocab/habitat/d1e594a1900"/>
      <skos:narrowMatch rdf:resource="http://104.244.76.201/Bionet-ANDS-test/vocab/habitat/d1e595a1900"/>
      <skos:narrowMatch rdf:resource="http://104.244.76.201/Bionet-ANDS-test/vocab/habitat/d1e597a1900"/>
      <skos:narrowMatch rdf:resource="http://104.244.76.201/Bionet-ANDS-test/vocab/habitat/d1e598a1900"/>
      <skos:narrowMatch rdf:resource="http://104.244.76.201/Bionet-ANDS-test/vocab/habitat/d1e599a1900"/>
      <skos:narrowMatch rdf:resource="http://104.244.76.201/Bionet-ANDS-test/vocab/habitat/d1e600a1900"/>
      <skos:narrowMatch rdf:resource="http://104.244.76.201/Bionet-ANDS-test/vocab/habitat/d1e601a1900"/>
      <skos:narrowMatch rdf:resource="http://104.244.76.201/Bionet-ANDS-test/vocab/habitat/d1e602a1900"/>
      <skos:narrowMatch rdf:resource="http://104.244.76.201/Bionet-ANDS-test/vocab/habitat/d1e603a1900"/>
      <skos:narrowMatch rdf:resource="http://104.244.76.201/Bionet-ANDS-test/vocab/habitat/d1e604a1900"/>
      <skos:narrowMatch rdf:resource="http://104.244.76.201/Bionet-ANDS-test/vocab/habitat/d1e605a1900"/>
      <skos:narrowMatch rdf:resource="http://104.244.76.201/Bionet-ANDS-test/vocab/habitat/d1e606a1900"/>
      <skos:narrowMatch rdf:resource="http://104.244.76.201/Bionet-ANDS-test/vocab/habitat/d1e607a1900"/>
      <skos:narrowMatch rdf:resource="http://104.244.76.201/Bionet-ANDS-test/vocab/habitat/d1e609a1900"/>
      <skos:narrowMatch rdf:resource="http://104.244.76.201/Bionet-ANDS-test/vocab/habitat/d1e610a1900"/>
      <skos:narrowMatch rdf:resource="http://104.244.76.201/Bionet-ANDS-test/vocab/habitat/d1e611a1900"/>
      <skos:narrowMatch rdf:resource="http://104.244.76.201/Bionet-ANDS-test/vocab/habitat/d1e612a1900"/>
      <skos:narrowMatch rdf:resource="http://104.244.76.201/Bionet-ANDS-test/vocab/habitat/d1e613a1900"/>
      <skos:narrowMatch rdf:resource="http://104.244.76.201/Bionet-ANDS-test/vocab/habitat/d1e614a1900"/>
      <skos:narrowMatch rdf:resource="http://104.244.76.201/Bionet-ANDS-test/vocab/habitat/d1e615a1900"/>
      <skos:narrowMatch rdf:resource="http://104.244.76.201/Bionet-ANDS-test/vocab/habitat/d1e616a1900"/>
      <skos:narrowMatch rdf:resource="http://104.244.76.201/Bionet-ANDS-test/vocab/habitat/d1e617a1900"/>
      <skos:narrowMatch rdf:resource="http://104.244.76.201/Bionet-ANDS-test/vocab/habitat/d1e618a1900"/>
      <skos:narrowMatch rdf:resource="http://104.244.76.201/Bionet-ANDS-test/vocab/habitat/d1e619a1900"/>
      <skos:narrowMatch rdf:resource="http://104.244.76.201/Bionet-ANDS-test/vocab/habitat/d1e621a1900"/>
      <skos:narrowMatch rdf:resource="http://104.244.76.201/Bionet-ANDS-test/vocab/habitat/d1e622a1900"/>
      <skos:narrowMatch rdf:resource="http://104.244.76.201/Bionet-ANDS-test/vocab/habitat/d1e623a1900"/>
      <skos:narrowMatch rdf:resource="http://104.244.76.201/Bionet-ANDS-test/vocab/habitat/d1e624a1900"/>
      <skos:narrowMatch rdf:resource="http://104.244.76.201/Bionet-ANDS-test/vocab/habitat/d1e625a1900"/>
      <skos:narrowMatch rdf:resource="http://104.244.76.201/Bionet-ANDS-test/vocab/habitat/d1e626a1900"/>
      <skos:narrowMatch rdf:resource="http://104.244.76.201/Bionet-ANDS-test/vocab/habitat/d1e627a1900"/>
      <skos:narrowMatch rdf:resource="http://104.244.76.201/Bionet-ANDS-test/vocab/habitat/d1e628a1900"/>
      <skos:narrowMatch rdf:resource="http://104.244.76.201/Bionet-ANDS-test/vocab/habitat/d1e629a1900"/>
      <skos:narrowMatch rdf:resource="http://104.244.76.201/Bionet-ANDS-test/vocab/habitat/d1e630a1900"/>
      <skos:narrowMatch rdf:resource="http://104.244.76.201/Bionet-ANDS-test/vocab/habitat/d1e631a1900"/>
      <skos:narrowMatch rdf:resource="http://104.244.76.201/Bionet-ANDS-test/vocab/habitat/d1e633a1900"/>
      <skos:narrowMatch rdf:resource="http://104.244.76.201/Bionet-ANDS-test/vocab/habitat/d1e634a1900"/>
      <skos:narrowMatch rdf:resource="http://104.244.76.201/Bionet-ANDS-test/vocab/habitat/d1e635a1900"/>
      <skos:narrowMatch rdf:resource="http://104.244.76.201/Bionet-ANDS-test/vocab/habitat/d1e636a1900"/>
      <skos:narrowMatch rdf:resource="http://104.244.76.201/Bionet-ANDS-test/vocab/habitat/d1e637a1900"/>
      <skos:narrowMatch rdf:resource="http://104.244.76.201/Bionet-ANDS-test/vocab/habitat/d1e638a1900"/>
      <skos:narrowMatch rdf:resource="http://104.244.76.201/Bionet-ANDS-test/vocab/habitat/d1e639a1900"/>
      <skos:narrowMatch rdf:resource="http://104.244.76.201/Bionet-ANDS-test/vocab/habitat/d1e640a1900"/>
      <skos:narrowMatch rdf:resource="http://104.244.76.201/Bionet-ANDS-test/vocab/habitat/d1e641a1900"/>
      <skos:narrowMatch rdf:resource="http://104.244.76.201/Bionet-ANDS-test/vocab/habitat/d1e642a1900"/>
      <skos:narrowMatch rdf:resource="http://104.244.76.201/Bionet-ANDS-test/vocab/habitat/d1e643a1900"/>
      <skos:narrowMatch rdf:resource="http://104.244.76.201/Bionet-ANDS-test/vocab/habitat/d1e645a1900"/>
      <skos:narrowMatch rdf:resource="http://104.244.76.201/Bionet-ANDS-test/vocab/habitat/d1e646a1900"/>
      <skos:narrowMatch rdf:resource="http://104.244.76.201/Bionet-ANDS-test/vocab/habitat/d1e647a1900"/>
      <skos:narrowMatch rdf:resource="http://104.244.76.201/Bionet-ANDS-test/vocab/habitat/d1e648a1900"/>
      <skos:narrowMatch rdf:resource="http://104.244.76.201/Bionet-ANDS-test/vocab/habitat/d1e649a1900"/>
      <skos:narrowMatch rdf:resource="http://104.244.76.201/Bionet-ANDS-test/vocab/habitat/d1e650a1900"/>
      <skos:definition xml:lang="en">A category or description of the habitat in which the Event occurred as per the following controlled vocabulary:</skos:definition>
      <skos:example xml:lang="en">“Sod grassland”, “Open tussock grassland”</skos:example>
   </rdf:Description>

   <rdf:Description rdf:about="http://104.244.76.201/Bionet-ANDS-test/schema/d1e651a1900">
      <rdf:type rdf:resource="http://www.w3.org/2004/02/skos/core#Concept"/>
      <skos:prefLabel xml:lang="en">samplingEffort</skos:prefLabel>
      <dcterms:creator>Bionet (NSW Office of Environment and Heritage)</dcterms:creator>
      <dcterms:contributor>Bionet (NSW Office of Environment and Heritage)</dcterms:contributor>
      <skos:broader rdf:resource="http://104.244.76.201/Bionet-ANDS-test/schema/d1e494a1900"/>
      <skos:definition xml:lang="en">The amount of effort expended during an Event.</skos:definition>
      <skos:example xml:lang="en">“60.00 Trap Nights”</skos:example>
   </rdf:Description>

   <rdf:Description rdf:about="http://104.244.76.201/Bionet-ANDS-test/schema/d1e656a1900">
      <rdf:type rdf:resource="http://www.w3.org/2004/02/skos/core#Concept"/>
      <skos:prefLabel xml:lang="en">samplingProtocol</skos:prefLabel>
      <dcterms:creator>Bionet (NSW Office of Environment and Heritage)</dcterms:creator>
      <dcterms:contributor>Bionet (NSW Office of Environment and Heritage)</dcterms:contributor>
      <skos:broader rdf:resource="http://104.244.76.201/Bionet-ANDS-test/schema/d1e494a1900"/>
      <skos:definition xml:lang="en">The name of, reference to, or description of the method or protocol used during an Event.</skos:definition>
      <skos:example xml:lang="en">“20 by 20 Vegetation Plot (old type)”, “Bat Ultrasound”, “Cage Trapping”</skos:example>
   </rdf:Description>

   <rdf:Description rdf:about="http://104.244.76.201/Bionet-ANDS-test/schema/d1e662a1900">
      <rdf:type rdf:resource="http://www.w3.org/2004/02/skos/core#Concept"/>
      <skos:prefLabel xml:lang="en">coordinatePrecision</skos:prefLabel>
      <dcterms:creator>Bionet (NSW Office of Environment and Heritage)</dcterms:creator>
      <dcterms:contributor>Bionet (NSW Office of Environment and Heritage)</dcterms:contributor>
      <skos:broader rdf:resource="http://104.244.76.201/Bionet-ANDS-test/schema/d1e661a1900"/>
      <skos:definition xml:lang="en">A decimal representation of the precision of the coordinates given in the decimalLatitude and decimalLongitude. For example, 2 for coordinates accurate to two decimal places.</skos:definition>
      <skos:definition xml:lang="en">Note: be careful with coordinates converted from D:M:S they can have a lot of decimal places that are not warranted by the original coordinates</skos:definition>
      <skos:example xml:lang="en">"1", “2”, “9”</skos:example>
   </rdf:Description>

   <rdf:Description rdf:about="http://104.244.76.201/Bionet-ANDS-test/schema/d1e669a1900">
      <rdf:type rdf:resource="http://www.w3.org/2004/02/skos/core#Concept"/>
      <skos:prefLabel xml:lang="en">coordinateUncertaintyInMeters</skos:prefLabel>
      <dcterms:creator>Bionet (NSW Office of Environment and Heritage)</dcterms:creator>
      <dcterms:contributor>Bionet (NSW Office of Environment and Heritage)</dcterms:contributor>
      <skos:broader rdf:resource="http://104.244.76.201/Bionet-ANDS-test/schema/d1e661a1900"/>
      <skos:definition xml:lang="en">The horizontal distance (in meters) from the given decimalLatitude and decimalLongitude describing the smallest circle within which the Location is likely to occur.</skos:definition>
      <skos:definition xml:lang="en">For example a value of 100 would mean that the location is accurate to the nearest 100 metres.</skos:definition>
      <skos:example xml:lang="en">"30.0000"</skos:example>
   </rdf:Description>

   <rdf:Description rdf:about="http://104.244.76.201/Bionet-ANDS-test/schema/d1e676a1900">
      <rdf:type rdf:resource="http://www.w3.org/2004/02/skos/core#Concept"/>
      <skos:prefLabel xml:lang="en">country</skos:prefLabel>
      <dcterms:creator>Bionet (NSW Office of Environment and Heritage)</dcterms:creator>
      <dcterms:contributor>Bionet (NSW Office of Environment and Heritage)</dcterms:contributor>
      <skos:broader rdf:resource="http://104.244.76.201/Bionet-ANDS-test/schema/d1e661a1900"/>
      <skos:definition xml:lang="en">The name of the country or major administrative unit in which the Location occurs. Recommended best practice is to use a controlled vocabulary such as the Getty Thesaurus of Geographic Names.</skos:definition>
      <skos:example xml:lang="en">"Australia”</skos:example>
   </rdf:Description>

   <rdf:Description rdf:about="http://104.244.76.201/Bionet-ANDS-test/schema/d1e681a1900">
      <rdf:type rdf:resource="http://www.w3.org/2004/02/skos/core#Concept"/>
      <skos:prefLabel xml:lang="en">countryCode</skos:prefLabel>
      <dcterms:creator>Bionet (NSW Office of Environment and Heritage)</dcterms:creator>
      <dcterms:contributor>Bionet (NSW Office of Environment and Heritage)</dcterms:contributor>
      <skos:broader rdf:resource="http://104.244.76.201/Bionet-ANDS-test/schema/d1e661a1900"/>
      <skos:definition xml:lang="en">The standard code for the country in which the Location occurs. Recommended best practice is to use ISO 3166-1-alpha-2 country codes.</skos:definition>
      <skos:example xml:lang="en">"AU” for Australia</skos:example>
   </rdf:Description>

   <rdf:Description rdf:about="http://104.244.76.201/Bionet-ANDS-test/schema/d1e686a1900">
      <rdf:type rdf:resource="http://www.w3.org/2004/02/skos/core#Concept"/>
      <skos:prefLabel xml:lang="en">county</skos:prefLabel>
      <dcterms:creator>Bionet (NSW Office of Environment and Heritage)</dcterms:creator>
      <dcterms:contributor>Bionet (NSW Office of Environment and Heritage)</dcterms:contributor>
      <skos:broader rdf:resource="http://104.244.76.201/Bionet-ANDS-test/schema/d1e661a1900"/>
      <skos:definition xml:lang="en">The full, unabbreviated name of the next smaller administrative region than stateProvince (county, shire, department, etc.) in which the Location occurs. In the context of NSW, the Local Government Area. Where the record does not occur in a NSW LGA this field give the value “N/A”</skos:definition>
      <skos:example xml:lang="en">"Clarence Valley”, “Dubbo”, “Tumut”</skos:example>
   </rdf:Description>

   <rdf:Description rdf:about="http://104.244.76.201/Bionet-ANDS-test/schema/d1e691a1900">
      <rdf:type rdf:resource="http://www.w3.org/2004/02/skos/core#Concept"/>
      <skos:prefLabel xml:lang="en">decimalLatitude</skos:prefLabel>
      <dcterms:creator>Bionet (NSW Office of Environment and Heritage)</dcterms:creator>
      <dcterms:contributor>Bionet (NSW Office of Environment and Heritage)</dcterms:contributor>
      <skos:broader rdf:resource="http://104.244.76.201/Bionet-ANDS-test/schema/d1e661a1900"/>
      <skos:definition xml:lang="en">The geographic latitude (in decimal degrees, using the spatial reference system given in geodeticDatum) of the geographic center of a Location. Positive values are north of the Equator, negative values are south of it. Legal values lie between -90 and 90, inclusive.</skos:definition>
      <skos:example xml:lang="en">"-41.0983423".</skos:example>
   </rdf:Description>

   <rdf:Description rdf:about="http://104.244.76.201/Bionet-ANDS-test/schema/d1e696a1900">
      <rdf:type rdf:resource="http://www.w3.org/2004/02/skos/core#Concept"/>
      <skos:prefLabel xml:lang="en">decimalLongitude</skos:prefLabel>
      <dcterms:creator>Bionet (NSW Office of Environment and Heritage)</dcterms:creator>
      <dcterms:contributor>Bionet (NSW Office of Environment and Heritage)</dcterms:contributor>
      <skos:broader rdf:resource="http://104.244.76.201/Bionet-ANDS-test/schema/d1e661a1900"/>
      <skos:definition xml:lang="en">The geographic longitude (in decimal degrees, using the spatial reference system given in geodeticDatum) of the geographic center of a Location. Positive values are east of the Greenwich Meridian, negative values are west of it. Legal values lie between -180 and 180, inclusive.</skos:definition>
      <skos:example xml:lang="en">"-121.1761111".</skos:example>
   </rdf:Description>

   <rdf:Description rdf:about="http://104.244.76.201/Bionet-ANDS-test/schema/d1e701a1900">
      <rdf:type rdf:resource="http://www.w3.org/2004/02/skos/core#Concept"/>
      <skos:prefLabel xml:lang="en">easting</skos:prefLabel>
      <dcterms:creator>Bionet (NSW Office of Environment and Heritage)</dcterms:creator>
      <dcterms:contributor>Bionet (NSW Office of Environment and Heritage)</dcterms:contributor>
      <skos:broader rdf:resource="http://104.244.76.201/Bionet-ANDS-test/schema/d1e661a1900"/>
      <skos:definition xml:lang="en">The reference in metres, measured east of an arbitrary origin (also referred to as the x-coordinate). The Easting provided in Atlas reports has been calculated from the Latitude and Longitude values. Data provided in MGA.</skos:definition>
      <skos:example xml:lang="en">“691573”</skos:example>
   </rdf:Description>

   <rdf:Description rdf:about="http://104.244.76.201/Bionet-ANDS-test/schema/d1e706a1900">
      <rdf:type rdf:resource="http://www.w3.org/2004/02/skos/core#Concept"/>
      <skos:prefLabel xml:lang="en">geodeticDatum</skos:prefLabel>
      <dcterms:creator>Bionet (NSW Office of Environment and Heritage)</dcterms:creator>
      <dcterms:contributor>Bionet (NSW Office of Environment and Heritage)</dcterms:contributor>
      <skos:broader rdf:resource="http://104.244.76.201/Bionet-ANDS-test/schema/d1e661a1900"/>
      <skos:definition xml:lang="en">The ellipsoid, geodetic datum, or spatial reference system (SRS) upon which the geographic coordinates given in decimalLatitude and decimalLongitude are based. Recommended best practice is to use the European Petroleum Survey Group (EPSG) code as a controlled vocabulary to provide an SRS, if known. Otherwise use a controlled vocabulary for the name or code of the geodetic datum, if known. Otherwise use a controlled vocabulary for the name or code of the ellipsoid, if known. If none of these is known, use the value "unknown".</skos:definition>
      <skos:example xml:lang="en">“GDA94”</skos:example>
   </rdf:Description>

   <rdf:Description rdf:about="http://104.244.76.201/Bionet-ANDS-test/schema/d1e711a1900">
      <rdf:type rdf:resource="http://www.w3.org/2004/02/skos/core#Concept"/>
      <skos:prefLabel xml:lang="en">georeferenceProtocol</skos:prefLabel>
      <dcterms:creator>Bionet (NSW Office of Environment and Heritage)</dcterms:creator>
      <dcterms:contributor>Bionet (NSW Office of Environment and Heritage)</dcterms:contributor>
      <skos:broader rdf:resource="http://104.244.76.201/Bionet-ANDS-test/schema/d1e661a1900"/>
      <skos:definition xml:lang="en">A description or reference to the methods used to determine the spatial footprint, coordinates, and uncertainties.</skos:definition>
      <skos:definition xml:lang="en">In the context of this data set, it will indicate if GPS was used to determine the location.</skos:definition>
      <skos:example xml:lang="en">“GPS”</skos:example>
   </rdf:Description>

   <rdf:Description rdf:about="http://104.244.76.201/Bionet-ANDS-test/schema/d1e718a1900">
      <rdf:type rdf:resource="http://www.w3.org/2004/02/skos/core#Concept"/>
      <skos:prefLabel xml:lang="en">locality</skos:prefLabel>
      <dcterms:creator>Bionet (NSW Office of Environment and Heritage)</dcterms:creator>
      <dcterms:contributor>Bionet (NSW Office of Environment and Heritage)</dcterms:contributor>
      <skos:broader rdf:resource="http://104.244.76.201/Bionet-ANDS-test/schema/d1e661a1900"/>
      <skos:definition xml:lang="en">The specific description of the place. Less specific geographic information can be provided in other geographic terms (higherGeography, continent, country, stateProvince, county, municipality, waterBody, island, islandGroup). This term may contain information modified from the original to correct perceived errors or standardize the description.</skos:definition>
      <skos:example xml:lang="en">“Hawkshead Road, 1km W of Hereford Park. Specified Map No: 8824”</skos:example>
   </rdf:Description>

   <rdf:Description rdf:about="http://104.244.76.201/Bionet-ANDS-test/schema/d1e724a1900">
      <rdf:type rdf:resource="http://www.w3.org/2004/02/skos/core#Concept"/>
      <skos:prefLabel xml:lang="en">locationID</skos:prefLabel>
      <dcterms:creator>Bionet (NSW Office of Environment and Heritage)</dcterms:creator>
      <dcterms:contributor>Bionet (NSW Office of Environment and Heritage)</dcterms:contributor>
      <skos:broader rdf:resource="http://104.244.76.201/Bionet-ANDS-test/schema/d1e661a1900"/>
      <skos:definition xml:lang="en">An identifier for the set of location information (data associated with dcterms:Location). May be a global unique identifier or an identifier specific to the data set.</skos:definition>
      <skos:example xml:lang="en">“7457-HO”, “5224-035”</skos:example>
   </rdf:Description>

   <rdf:Description rdf:about="http://104.244.76.201/Bionet-ANDS-test/schema/d1e729a1900">
      <rdf:type rdf:resource="http://www.w3.org/2004/02/skos/core#Concept"/>
      <skos:prefLabel xml:lang="en">locationRemarks</skos:prefLabel>
      <dcterms:creator>Bionet (NSW Office of Environment and Heritage)</dcterms:creator>
      <dcterms:contributor>Bionet (NSW Office of Environment and Heritage)</dcterms:contributor>
      <skos:broader rdf:resource="http://104.244.76.201/Bionet-ANDS-test/schema/d1e661a1900"/>
      <skos:definition xml:lang="en">Comments or notes about the Location.</skos:definition>
      <skos:example xml:lang="en">“Partially cleared and regenerated.”</skos:example>
   </rdf:Description>

   <rdf:Description rdf:about="http://104.244.76.201/Bionet-ANDS-test/schema/d1e734a1900">
      <rdf:type rdf:resource="http://www.w3.org/2004/02/skos/core#Concept"/>
      <skos:prefLabel xml:lang="en">mapSheetNumber</skos:prefLabel>
      <dcterms:creator>Bionet (NSW Office of Environment and Heritage)</dcterms:creator>
      <dcterms:contributor>Bionet (NSW Office of Environment and Heritage)</dcterms:contributor>
      <skos:broader rdf:resource="http://104.244.76.201/Bionet-ANDS-test/schema/d1e661a1900"/>
      <skos:definition xml:lang="en">The Australian Topographic Map Sheet number for the map which covers the location of the record.  Where the record does not overlap a valid NSW mapsheet this field gives the value “N/A”</skos:definition>
      <skos:example xml:lang="en">“8824 – BEGA”</skos:example>
   </rdf:Description>

   <rdf:Description rdf:about="http://104.244.76.201/Bionet-ANDS-test/schema/d1e739a1900">
      <rdf:type rdf:resource="http://www.w3.org/2004/02/skos/core#Concept"/>
      <skos:prefLabel xml:lang="en">maximumElevationInMeters</skos:prefLabel>
      <dcterms:creator>Bionet (NSW Office of Environment and Heritage)</dcterms:creator>
      <dcterms:contributor>Bionet (NSW Office of Environment and Heritage)</dcterms:contributor>
      <skos:broader rdf:resource="http://104.244.76.201/Bionet-ANDS-test/schema/d1e661a1900"/>
      <skos:definition xml:lang="en">The upper limit of the range of elevation (altitude, usually above sea level), in meters.</skos:definition>
      <skos:example xml:lang="en">"200".</skos:example>
   </rdf:Description>

   <rdf:Description rdf:about="http://104.244.76.201/Bionet-ANDS-test/schema/d1e744a1900">
      <rdf:type rdf:resource="http://www.w3.org/2004/02/skos/core#Concept"/>
      <skos:prefLabel xml:lang="en">minimumElevationInMeters</skos:prefLabel>
      <dcterms:creator>Bionet (NSW Office of Environment and Heritage)</dcterms:creator>
      <dcterms:contributor>Bionet (NSW Office of Environment and Heritage)</dcterms:contributor>
      <skos:broader rdf:resource="http://104.244.76.201/Bionet-ANDS-test/schema/d1e661a1900"/>
      <skos:definition xml:lang="en">The lower limit of the range of elevation (altitude, usually above sea level), in meters.</skos:definition>
      <skos:example xml:lang="en">"100".</skos:example>
   </rdf:Description>

   <rdf:Description rdf:about="http://104.244.76.201/Bionet-ANDS-test/schema/d1e749a1900">
      <rdf:type rdf:resource="http://www.w3.org/2004/02/skos/core#Concept"/>
      <skos:prefLabel xml:lang="en">northing</skos:prefLabel>
      <dcterms:creator>Bionet (NSW Office of Environment and Heritage)</dcterms:creator>
      <dcterms:contributor>Bionet (NSW Office of Environment and Heritage)</dcterms:contributor>
      <skos:broader rdf:resource="http://104.244.76.201/Bionet-ANDS-test/schema/d1e661a1900"/>
      <skos:definition xml:lang="en">The reference in metres, measured north of an arbitrary origin (also referred to as the y-coordinate). The Northing provided in Atlas reports has been calculated from the Latitude and Longitude values. Data provided in Map Grid of Australia (MGA).</skos:definition>
      <skos:example xml:lang="en">“6121614”</skos:example>
   </rdf:Description>

   <rdf:Description rdf:about="http://104.244.76.201/Bionet-ANDS-test/schema/d1e754a1900">
      <rdf:type rdf:resource="http://www.w3.org/2004/02/skos/core#Concept"/>
      <skos:prefLabel xml:lang="en">stateProvince</skos:prefLabel>
      <dcterms:creator>Bionet (NSW Office of Environment and Heritage)</dcterms:creator>
      <dcterms:contributor>Bionet (NSW Office of Environment and Heritage)</dcterms:contributor>
      <skos:broader rdf:resource="http://104.244.76.201/Bionet-ANDS-test/schema/d1e661a1900"/>
      <skos:definition xml:lang="en">The name of the next smaller administrative region than country (state, province, canton, department, region, etc.) in which the Location occurs.  Where the record does not overlap a valid Australian state, this field gives the value “N/A”</skos:definition>
      <skos:example xml:lang="en">"NSW”</skos:example>
   </rdf:Description>

   <rdf:Description rdf:about="http://104.244.76.201/Bionet-ANDS-test/schema/d1e759a1900">
      <rdf:type rdf:resource="http://www.w3.org/2004/02/skos/core#Concept"/>
      <skos:prefLabel xml:lang="en">zone</skos:prefLabel>
      <dcterms:creator>Bionet (NSW Office of Environment and Heritage)</dcterms:creator>
      <dcterms:contributor>Bionet (NSW Office of Environment and Heritage)</dcterms:contributor>
      <skos:broader rdf:resource="http://104.244.76.201/Bionet-ANDS-test/schema/d1e661a1900"/>
      <skos:definition xml:lang="en">A 6° band of longitude, divided according to the Universal Transverse Mercator (UTM) coordinate system. NSW Is divided into 4 Zones; Zone 56 is 150° –156° longitude, which encompasses much of eastern NSW. Zone 55 is 144°–150° longitude. Zone 54 is 138°–144° longitude, encompassing most of Western NSW. Zone 57 covers Lord Howe Island. The Zone in Atlas reports has been calculated from the Latitude and Longitude values. Data provided in MGA.</skos:definition>
      <skos:example xml:lang="en">“55”</skos:example>
   </rdf:Description>

   <rdf:Description rdf:about="http://104.244.76.201/Bionet-ANDS-test/schema/d1e765a1900">
      <rdf:type rdf:resource="http://www.w3.org/2004/02/skos/core#Concept"/>
      <skos:prefLabel xml:lang="en">class</skos:prefLabel>
      <dcterms:creator>Bionet (NSW Office of Environment and Heritage)</dcterms:creator>
      <dcterms:contributor>Bionet (NSW Office of Environment and Heritage)</dcterms:contributor>
      <skos:broader rdf:resource="http://104.244.76.201/Bionet-ANDS-test/schema/d1e764a1900"/>
      <skos:definition xml:lang="en">The full scientific name of the class in which the taxon is classified.</skos:definition>
      <skos:example xml:lang="en">"Aves", "Equisetopsida"</skos:example>
   </rdf:Description>

   <rdf:Description rdf:about="http://104.244.76.201/Bionet-ANDS-test/schema/d1e770a1900">
      <rdf:type rdf:resource="http://www.w3.org/2004/02/skos/core#Concept"/>
      <skos:prefLabel xml:lang="en">family</skos:prefLabel>
      <dcterms:creator>Bionet (NSW Office of Environment and Heritage)</dcterms:creator>
      <dcterms:contributor>Bionet (NSW Office of Environment and Heritage)</dcterms:contributor>
      <skos:broader rdf:resource="http://104.244.76.201/Bionet-ANDS-test/schema/d1e764a1900"/>
      <skos:definition xml:lang="en">The full scientific name of the family in which the taxon is classified.</skos:definition>
      <skos:example xml:lang="en">"Cacatuidae", "Fabaceae"</skos:example>
   </rdf:Description>

   <rdf:Description rdf:about="http://104.244.76.201/Bionet-ANDS-test/schema/d1e775a1900">
      <rdf:type rdf:resource="http://www.w3.org/2004/02/skos/core#Concept"/>
      <skos:prefLabel xml:lang="en">genus</skos:prefLabel>
      <dcterms:creator>Bionet (NSW Office of Environment and Heritage)</dcterms:creator>
      <dcterms:contributor>Bionet (NSW Office of Environment and Heritage)</dcterms:contributor>
      <skos:broader rdf:resource="http://104.244.76.201/Bionet-ANDS-test/schema/d1e764a1900"/>
      <skos:definition xml:lang="en">The full scientific name of the genus in which the taxon is classified.</skos:definition>
      <skos:example xml:lang="en">"Callocephalon", "Acacia"</skos:example>
   </rdf:Description>

   <rdf:Description rdf:about="http://104.244.76.201/Bionet-ANDS-test/schema/d1e780a1900">
      <rdf:type rdf:resource="http://www.w3.org/2004/02/skos/core#Concept"/>
      <skos:prefLabel xml:lang="en">infraspecificEpithet</skos:prefLabel>
      <dcterms:creator>Bionet (NSW Office of Environment and Heritage)</dcterms:creator>
      <dcterms:contributor>Bionet (NSW Office of Environment and Heritage)</dcterms:contributor>
      <skos:broader rdf:resource="http://104.244.76.201/Bionet-ANDS-test/schema/d1e764a1900"/>
      <skos:definition xml:lang="en">The name of the lowest or terminal infraspecific epithet of the scientificName, excluding any rank designation.</skos:definition>
      <skos:example xml:lang="en">"latifolia", "parviflora"</skos:example>
   </rdf:Description>

   <rdf:Description rdf:about="http://104.244.76.201/Bionet-ANDS-test/schema/d1e785a1900">
      <rdf:type rdf:resource="http://www.w3.org/2004/02/skos/core#Concept"/>
      <skos:prefLabel xml:lang="en">kingdom</skos:prefLabel>
      <dcterms:creator>Bionet (NSW Office of Environment and Heritage)</dcterms:creator>
      <dcterms:contributor>Bionet (NSW Office of Environment and Heritage)</dcterms:contributor>
      <skos:broader rdf:resource="http://104.244.76.201/Bionet-ANDS-test/schema/d1e764a1900"/>
      <skos:narrowMatch rdf:resource="http://104.244.76.201/Bionet-ANDS-test/vocab/kingdom/d1e791a1900"/>
      <skos:narrowMatch rdf:resource="http://104.244.76.201/Bionet-ANDS-test/vocab/kingdom/d1e792a1900"/>
      <skos:narrowMatch rdf:resource="http://104.244.76.201/Bionet-ANDS-test/vocab/kingdom/d1e793a1900"/>
      <skos:definition xml:lang="en">One of the following three values:</skos:definition>
      <skos:example xml:lang="en">"Plantae",</skos:example>
   </rdf:Description>

   <rdf:Description rdf:about="http://104.244.76.201/Bionet-ANDS-test/schema/d1e794a1900">
      <rdf:type rdf:resource="http://www.w3.org/2004/02/skos/core#Concept"/>
      <skos:prefLabel xml:lang="en">nomenclaturalCode</skos:prefLabel>
      <dcterms:creator>Bionet (NSW Office of Environment and Heritage)</dcterms:creator>
      <dcterms:contributor>Bionet (NSW Office of Environment and Heritage)</dcterms:contributor>
      <skos:broader rdf:resource="http://104.244.76.201/Bionet-ANDS-test/schema/d1e764a1900"/>
      <skos:definition xml:lang="en">The nomenclatural code (or codes in the case of an ambiregnal name) under which the scientificName is constructed. Recommended best practice is to use a controlled vocabulary.</skos:definition>
      <skos:example xml:lang="en">"ICBN", "ICZN"</skos:example>
   </rdf:Description>

   <rdf:Description rdf:about="http://104.244.76.201/Bionet-ANDS-test/schema/d1e799a1900">
      <rdf:type rdf:resource="http://www.w3.org/2004/02/skos/core#Concept"/>
      <skos:prefLabel xml:lang="en">order</skos:prefLabel>
      <dcterms:creator>Bionet (NSW Office of Environment and Heritage)</dcterms:creator>
      <dcterms:contributor>Bionet (NSW Office of Environment and Heritage)</dcterms:contributor>
      <skos:broader rdf:resource="http://104.244.76.201/Bionet-ANDS-test/schema/d1e764a1900"/>
      <skos:definition xml:lang="en">The full scientific name of the order in which the taxon is classified.</skos:definition>
      <skos:example xml:lang="en">"Psittaciformes"</skos:example>
   </rdf:Description>

   <rdf:Description rdf:about="http://104.244.76.201/Bionet-ANDS-test/schema/d1e804a1900">
      <rdf:type rdf:resource="http://www.w3.org/2004/02/skos/core#Concept"/>
      <skos:prefLabel xml:lang="en">scientificName</skos:prefLabel>
      <dcterms:creator>Bionet (NSW Office of Environment and Heritage)</dcterms:creator>
      <dcterms:contributor>Bionet (NSW Office of Environment and Heritage)</dcterms:contributor>
      <skos:broader rdf:resource="http://104.244.76.201/Bionet-ANDS-test/schema/d1e764a1900"/>
      <skos:definition xml:lang="en">The full scientific name, with authorship and date information if known. When forming part of an identification, this should be the name in lowest level taxonomic rank that can be determined.</skos:definition>
      <skos:example xml:lang="en">"Callocephalon fimbriatum”, “Acacia pycnantha”</skos:example>
   </rdf:Description>

   <rdf:Description rdf:about="http://104.244.76.201/Bionet-ANDS-test/schema/d1e809a1900">
      <rdf:type rdf:resource="http://www.w3.org/2004/02/skos/core#Concept"/>
      <skos:prefLabel xml:lang="en">scientificNameAuthorship</skos:prefLabel>
      <dcterms:creator>Bionet (NSW Office of Environment and Heritage)</dcterms:creator>
      <dcterms:contributor>Bionet (NSW Office of Environment and Heritage)</dcterms:contributor>
      <skos:broader rdf:resource="http://104.244.76.201/Bionet-ANDS-test/schema/d1e764a1900"/>
      <skos:definition xml:lang="en">The authorship information for the scientificName formatted according to the conventions of the applicable nomenclaturalCode.</skos:definition>
      <skos:example xml:lang="en">“(Grant, 1803)”</skos:example>
   </rdf:Description>

   <rdf:Description rdf:about="http://104.244.76.201/Bionet-ANDS-test/schema/d1e814a1900">
      <rdf:type rdf:resource="http://www.w3.org/2004/02/skos/core#Concept"/>
      <skos:prefLabel xml:lang="en">scientificNameID</skos:prefLabel>
      <dcterms:creator>Bionet (NSW Office of Environment and Heritage)</dcterms:creator>
      <dcterms:contributor>Bionet (NSW Office of Environment and Heritage)</dcterms:contributor>
      <skos:broader rdf:resource="http://104.244.76.201/Bionet-ANDS-test/schema/d1e764a1900"/>
      <skos:definition xml:lang="en">An identifier for the nomenclatural (not taxonomic) details of a scientific name.</skos:definition>
      <skos:example xml:lang="en">“0268”</skos:example>
   </rdf:Description>

   <rdf:Description rdf:about="http://104.244.76.201/Bionet-ANDS-test/schema/d1e819a1900">
      <rdf:type rdf:resource="http://www.w3.org/2004/02/skos/core#Concept"/>
      <skos:prefLabel xml:lang="en">sortOrder</skos:prefLabel>
      <dcterms:creator>Bionet (NSW Office of Environment and Heritage)</dcterms:creator>
      <dcterms:contributor>Bionet (NSW Office of Environment and Heritage)</dcterms:contributor>
      <skos:broader rdf:resource="http://104.244.76.201/Bionet-ANDS-test/schema/d1e764a1900"/>
      <skos:definition xml:lang="en">An integer used to sort species in a sensible taxonomic order</skos:definition>
      <skos:example xml:lang="en">“97”</skos:example>
   </rdf:Description>

   <rdf:Description rdf:about="http://104.244.76.201/Bionet-ANDS-test/schema/d1e825a1900">
      <rdf:type rdf:resource="http://www.w3.org/2004/02/skos/core#Concept"/>
      <skos:prefLabel xml:lang="en">specificEpithet</skos:prefLabel>
      <dcterms:creator>Bionet (NSW Office of Environment and Heritage)</dcterms:creator>
      <dcterms:contributor>Bionet (NSW Office of Environment and Heritage)</dcterms:contributor>
      <skos:broader rdf:resource="http://104.244.76.201/Bionet-ANDS-test/schema/d1e764a1900"/>
      <skos:definition xml:lang="en">The name of the first or species epithet of the scientificName.</skos:definition>
      <skos:example xml:lang="en">"fimbriatum", "pycnantha"</skos:example>
   </rdf:Description>

   <rdf:Description rdf:about="http://104.244.76.201/Bionet-ANDS-test/schema/d1e830a1900">
      <rdf:type rdf:resource="http://www.w3.org/2004/02/skos/core#Concept"/>
      <skos:prefLabel xml:lang="en">taxonRank</skos:prefLabel>
      <dcterms:creator>Bionet (NSW Office of Environment and Heritage)</dcterms:creator>
      <dcterms:contributor>Bionet (NSW Office of Environment and Heritage)</dcterms:contributor>
      <skos:broader rdf:resource="http://104.244.76.201/Bionet-ANDS-test/schema/d1e764a1900"/>
      <skos:definition xml:lang="en">The taxonomic rank of the most specific name in the scientificName.</skos:definition>
      <skos:example xml:lang="en">"Subspecies", "Species", "Genus".</skos:example>
   </rdf:Description>

   <rdf:Description rdf:about="http://104.244.76.201/Bionet-ANDS-test/schema/d1e835a1900">
      <rdf:type rdf:resource="http://www.w3.org/2004/02/skos/core#Concept"/>
      <skos:prefLabel xml:lang="en">vernacularName</skos:prefLabel>
      <dcterms:creator>Bionet (NSW Office of Environment and Heritage)</dcterms:creator>
      <dcterms:contributor>Bionet (NSW Office of Environment and Heritage)</dcterms:contributor>
      <skos:broader rdf:resource="http://104.244.76.201/Bionet-ANDS-test/schema/d1e764a1900"/>
      <skos:definition xml:lang="en">A common or vernacular name.</skos:definition>
      <skos:example xml:lang="en">"Gang-gang Cockatoo”, “Golden Wattle”</skos:example>
   </rdf:Description>

   <rdf:Description rdf:about="http://104.244.76.201/Bionet-ANDS-test/schema/d1e843a1900">
      <rdf:type rdf:resource="http://www.w3.org/2004/02/skos/core#Concept"/>
      <skos:prefLabel xml:lang="en">measurementType</skos:prefLabel>
      <dcterms:creator>Bionet (NSW Office of Environment and Heritage)</dcterms:creator>
      <dcterms:contributor>Bionet (NSW Office of Environment and Heritage)</dcterms:contributor>
      <skos:broader rdf:resource="http://104.244.76.201/Bionet-ANDS-test/schema/d1e840a1900"/>
      <skos:narrower rdf:resource="http://104.244.76.201/Bionet-ANDS-test/schema/d1e861a1900"/>
      <skos:narrower rdf:resource="http://104.244.76.201/Bionet-ANDS-test/schema/d1e866a1900"/>
      <skos:narrower rdf:resource="http://104.244.76.201/Bionet-ANDS-test/schema/d1e914a1900"/>
      <skos:narrower rdf:resource="http://104.244.76.201/Bionet-ANDS-test/schema/d1e919a1900"/>
      <skos:definition xml:lang="en">The nature of the measurement, fact, characteristic, or assertion. Recommended best practice is to use a controlled vocabulary.</skos:definition>
      <skos:definition xml:lang="en">See the meaurementType table below for the full list of measurements supplied via the Species Sightings Web Service</skos:definition>
      <skos:example xml:lang="en">“Aspect”</skos:example>
   </rdf:Description>

   <rdf:Description rdf:about="http://104.244.76.201/Bionet-ANDS-test/schema/d1e850a1900">
      <rdf:type rdf:resource="http://www.w3.org/2004/02/skos/core#Concept"/>
      <skos:prefLabel xml:lang="en">measurementValue</skos:prefLabel>
      <dcterms:creator>Bionet (NSW Office of Environment and Heritage)</dcterms:creator>
      <dcterms:contributor>Bionet (NSW Office of Environment and Heritage)</dcterms:contributor>
      <skos:broader rdf:resource="http://104.244.76.201/Bionet-ANDS-test/schema/d1e840a1900"/>
      <skos:definition xml:lang="en">The value of the measurement, fact, characteristic, or assertion.</skos:definition>
      <skos:example xml:lang="en">“30”</skos:example>
   </rdf:Description>

   <rdf:Description rdf:about="http://104.244.76.201/Bionet-ANDS-test/schema/d1e855a1900">
      <rdf:type rdf:resource="http://www.w3.org/2004/02/skos/core#Concept"/>
      <skos:prefLabel xml:lang="en">measurementUnit</skos:prefLabel>
      <dcterms:creator>Bionet (NSW Office of Environment and Heritage)</dcterms:creator>
      <dcterms:contributor>Bionet (NSW Office of Environment and Heritage)</dcterms:contributor>
      <skos:broader rdf:resource="http://104.244.76.201/Bionet-ANDS-test/schema/d1e840a1900"/>
      <skos:definition xml:lang="en">The units associated with the measurementValue. Recommended best practice is to use the International System of Units (SI).</skos:definition>
      <skos:example xml:lang="en">“degrees clockwise from true North”</skos:example>
   </rdf:Description>

   <rdf:Description rdf:about="http://104.244.76.201/Bionet-ANDS-test/schema/d1e106a1900">
      <rdf:type rdf:resource="http://www.w3.org/2004/02/skos/core#Concept"/>
      <skos:prefLabel xml:lang="en">BFMCS</skos:prefLabel>
      <dcterms:creator>Bionet (NSW Office of Environment and Heritage)</dcterms:creator>
      <dcterms:contributor>Bionet (NSW Office of Environment and Heritage)</dcterms:contributor>
      <skos:broader rdf:resource="http://104.244.76.201/Bionet-ANDS-test/schema/d1e81a1900"/>
      <skos:definition xml:lang="en">The number of bush fire management council areas that the species is found in.</skos:definition>
      <skos:example xml:lang="en">“8”</skos:example>
   </rdf:Description>

   <rdf:Description rdf:about="http://104.244.76.201/Bionet-ANDS-test/schema/d1e111a1900">
      <rdf:type rdf:resource="http://www.w3.org/2004/02/skos/core#Concept"/>
      <skos:prefLabel xml:lang="en">botanicalDivision</skos:prefLabel>
      <dcterms:creator>Bionet (NSW Office of Environment and Heritage)</dcterms:creator>
      <dcterms:contributor>Bionet (NSW Office of Environment and Heritage)</dcterms:contributor>
      <skos:broader rdf:resource="http://104.244.76.201/Bionet-ANDS-test/schema/d1e81a1900"/>
      <skos:narrowMatch rdf:resource="http://104.244.76.201/Bionet-ANDS-test/vocab/botanicalDivision/d1e117a1900"/>
      <skos:narrowMatch rdf:resource="http://104.244.76.201/Bionet-ANDS-test/vocab/botanicalDivision/d1e118a1900"/>
      <skos:narrowMatch rdf:resource="http://104.244.76.201/Bionet-ANDS-test/vocab/botanicalDivision/d1e119a1900"/>
      <skos:narrowMatch rdf:resource="http://104.244.76.201/Bionet-ANDS-test/vocab/botanicalDivision/d1e120a1900"/>
      <skos:narrowMatch rdf:resource="http://104.244.76.201/Bionet-ANDS-test/vocab/botanicalDivision/d1e121a1900"/>
      <skos:narrowMatch rdf:resource="http://104.244.76.201/Bionet-ANDS-test/vocab/botanicalDivision/d1e122a1900"/>
      <skos:narrowMatch rdf:resource="http://104.244.76.201/Bionet-ANDS-test/vocab/botanicalDivision/d1e123a1900"/>
      <skos:narrowMatch rdf:resource="http://104.244.76.201/Bionet-ANDS-test/vocab/botanicalDivision/d1e124a1900"/>
      <skos:narrowMatch rdf:resource="http://104.244.76.201/Bionet-ANDS-test/vocab/botanicalDivision/d1e125a1900"/>
      <skos:narrowMatch rdf:resource="http://104.244.76.201/Bionet-ANDS-test/vocab/botanicalDivision/d1e126a1900"/>
      <skos:narrowMatch rdf:resource="http://104.244.76.201/Bionet-ANDS-test/vocab/botanicalDivision/d1e127a1900"/>
      <skos:narrowMatch rdf:resource="http://104.244.76.201/Bionet-ANDS-test/vocab/botanicalDivision/d1e129a1900"/>
      <skos:definition xml:lang="en">The name of the Botanical Division within which the flora record occurs based on Harden (1990)[1]. Will be one of the following:</skos:definition>
      <skos:example xml:lang="en">“North Coast”</skos:example>
   </rdf:Description>

   <rdf:Description rdf:about="http://104.244.76.201/Bionet-ANDS-test/schema/d1e130a1900">
      <rdf:type rdf:resource="http://www.w3.org/2004/02/skos/core#Concept"/>
      <skos:prefLabel xml:lang="en">CMA</skos:prefLabel>
      <dcterms:creator>Bionet (NSW Office of Environment and Heritage)</dcterms:creator>
      <dcterms:contributor>Bionet (NSW Office of Environment and Heritage)</dcterms:contributor>
      <skos:broader rdf:resource="http://104.244.76.201/Bionet-ANDS-test/schema/d1e81a1900"/>
      <skos:definition xml:lang="en">The name of the Catchment Management Authority within which the record occurs.</skos:definition>
      <skos:example xml:lang="en">“Northern Rivers”</skos:example>
   </rdf:Description>

   <rdf:Description rdf:about="http://104.244.76.201/Bionet-ANDS-test/schema/d1e135a1900">
      <rdf:type rdf:resource="http://www.w3.org/2004/02/skos/core#Concept"/>
      <skos:prefLabel xml:lang="en">CMAsubregion</skos:prefLabel>
      <dcterms:creator>Bionet (NSW Office of Environment and Heritage)</dcterms:creator>
      <dcterms:contributor>Bionet (NSW Office of Environment and Heritage)</dcterms:contributor>
      <skos:broader rdf:resource="http://104.244.76.201/Bionet-ANDS-test/schema/d1e81a1900"/>
      <skos:definition xml:lang="en">The name of the Catchment Management Authority subregion within which the record occurs.</skos:definition>
      <skos:example xml:lang="en">“Clarence Valley”</skos:example>
   </rdf:Description>

   <rdf:Description rdf:about="http://104.244.76.201/Bionet-ANDS-test/schema/d1e140a1900">
      <rdf:type rdf:resource="http://www.w3.org/2004/02/skos/core#Concept"/>
      <skos:prefLabel xml:lang="en">floraReserve</skos:prefLabel>
      <dcterms:creator>Bionet (NSW Office of Environment and Heritage)</dcterms:creator>
      <dcterms:contributor>Bionet (NSW Office of Environment and Heritage)</dcterms:contributor>
      <skos:broader rdf:resource="http://104.244.76.201/Bionet-ANDS-test/schema/d1e81a1900"/>
      <skos:definition xml:lang="en">If the record occurs within a flora reserve (as defined in the Forestry Act 2012) this field gives the name of that flora reserve. If the field is marked “N/A” this indicates that the record does not occur within a flora reserve.</skos:definition>
      <skos:definition xml:lang="en">Note: This field does not give the name of reserves administered under the National Parks Wildlife Act 1974. See the ‘reserve’ field for information on reserves administered under that act.</skos:definition>
      <skos:example xml:lang="en">“Fenwicks Scrub Flora Reserve”</skos:example>
   </rdf:Description>

   <rdf:Description rdf:about="http://104.244.76.201/Bionet-ANDS-test/schema/d1e147a1900">
      <rdf:type rdf:resource="http://www.w3.org/2004/02/skos/core#Concept"/>
      <skos:prefLabel xml:lang="en">geogExtent</skos:prefLabel>
      <dcterms:creator>Bionet (NSW Office of Environment and Heritage)</dcterms:creator>
      <dcterms:contributor>Bionet (NSW Office of Environment and Heritage)</dcterms:contributor>
      <skos:broader rdf:resource="http://104.244.76.201/Bionet-ANDS-test/schema/d1e81a1900"/>
      <skos:narrowMatch rdf:resource="http://104.244.76.201/Bionet-ANDS-test/vocab/geogExtent/d1e155a1900"/>
      <skos:narrowMatch rdf:resource="http://104.244.76.201/Bionet-ANDS-test/vocab/geogExtent/d1e156a1900"/>
      <skos:narrowMatch rdf:resource="http://104.244.76.201/Bionet-ANDS-test/vocab/geogExtent/d1e157a1900"/>
      <skos:definition xml:lang="en">The geographic extent of the species based on the following controlled vocabulary:</skos:definition>
      <skos:definition xml:lang="en">Otherwise this field gives the value “N/A”</skos:definition>
      <skos:example xml:lang="en">“HR”</skos:example>
   </rdf:Description>

   <rdf:Description rdf:about="http://104.244.76.201/Bionet-ANDS-test/schema/d1e158a1900">
      <rdf:type rdf:resource="http://www.w3.org/2004/02/skos/core#Concept"/>
      <skos:prefLabel xml:lang="en">IBRA</skos:prefLabel>
      <dcterms:creator>Bionet (NSW Office of Environment and Heritage)</dcterms:creator>
      <dcterms:contributor>Bionet (NSW Office of Environment and Heritage)</dcterms:contributor>
      <skos:broader rdf:resource="http://104.244.76.201/Bionet-ANDS-test/schema/d1e81a1900"/>
      <skos:definition xml:lang="en">The name of the IRBA (Interim Biogeographic Regionalisation for Australia) Region within which the record occurs. This is based on IRBA version 6.1. Otherwise this field gives the value “N/A”</skos:definition>
      <skos:definition xml:lang="en">For more information on IBRA refer to:http://www.environment.gov.au/topics/land/national-reserve-system/science-maps-and-data/australias-bioregions-ibra</skos:definition>
      <skos:example xml:lang="en">“New England Tablelands”</skos:example>
   </rdf:Description>

   <rdf:Description rdf:about="http://104.244.76.201/Bionet-ANDS-test/schema/d1e165a1900">
      <rdf:type rdf:resource="http://www.w3.org/2004/02/skos/core#Concept"/>
      <skos:prefLabel xml:lang="en">mechanicalHRDescription</skos:prefLabel>
      <dcterms:creator>Bionet (NSW Office of Environment and Heritage)</dcterms:creator>
      <dcterms:contributor>Bionet (NSW Office of Environment and Heritage)</dcterms:contributor>
      <skos:broader rdf:resource="http://104.244.76.201/Bionet-ANDS-test/schema/d1e81a1900"/>
      <skos:definition xml:lang="en">Information on any restrictions on the use of Mechanical Hazard Reduction Techniques within 100 metres of the Occurrence record.  Otherwise this field gives the value “N/A”</skos:definition>
      <skos:example xml:lang="en">“No slashing, trittering or tree removal”, “Slashing in winter, but no trittering or tree removal”</skos:example>
   </rdf:Description>

   <rdf:Description rdf:about="http://104.244.76.201/Bionet-ANDS-test/schema/d1e170a1900">
      <rdf:type rdf:resource="http://www.w3.org/2004/02/skos/core#Concept"/>
      <skos:prefLabel xml:lang="en">potentialImpact</skos:prefLabel>
      <dcterms:creator>Bionet (NSW Office of Environment and Heritage)</dcterms:creator>
      <dcterms:contributor>Bionet (NSW Office of Environment and Heritage)</dcterms:contributor>
      <skos:broader rdf:resource="http://104.244.76.201/Bionet-ANDS-test/schema/d1e81a1900"/>
      <skos:narrowMatch rdf:resource="http://104.244.76.201/Bionet-ANDS-test/vocab/potentialImpact/d1e176a1900"/>
      <skos:narrowMatch rdf:resource="http://104.244.76.201/Bionet-ANDS-test/vocab/potentialImpact/d1e177a1900"/>
      <skos:narrowMatch rdf:resource="http://104.244.76.201/Bionet-ANDS-test/vocab/potentialImpact/d1e178a1900"/>
      <skos:narrowMatch rdf:resource="http://104.244.76.201/Bionet-ANDS-test/vocab/potentialImpact/d1e179a1900"/>
      <skos:definition xml:lang="en">A categorisation of the information recorded in SpeciesFireDiscription into one of three broad categories related to the use of fire as a Hazard Reduction techniques using the following controlled vocabulary:</skos:definition>
      <skos:example xml:lang="en">“Restrict Bush Fire”</skos:example>
   </rdf:Description>

   <rdf:Description rdf:about="http://104.244.76.201/Bionet-ANDS-test/schema/d1e180a1900">
      <rdf:type rdf:resource="http://www.w3.org/2004/02/skos/core#Concept"/>
      <skos:prefLabel xml:lang="en">profileID</skos:prefLabel>
      <dcterms:creator>Bionet (NSW Office of Environment and Heritage)</dcterms:creator>
      <dcterms:contributor>Bionet (NSW Office of Environment and Heritage)</dcterms:contributor>
      <skos:broader rdf:resource="http://104.244.76.201/Bionet-ANDS-test/schema/d1e81a1900"/>
      <skos:definition xml:lang="en">The unique identifier for the related threatened species profile as stored in the Threatened Species Profile Database maintained by the Office of Environment and Heritage. Otherwise this field gives the value “N/A”</skos:definition>
      <skos:example xml:lang="en">“10484”</skos:example>
   </rdf:Description>

   <rdf:Description rdf:about="http://104.244.76.201/Bionet-ANDS-test/schema/d1e186a1900">
      <rdf:type rdf:resource="http://www.w3.org/2004/02/skos/core#Concept"/>
      <skos:prefLabel xml:lang="en">reserve</skos:prefLabel>
      <dcterms:creator>Bionet (NSW Office of Environment and Heritage)</dcterms:creator>
      <dcterms:contributor>Bionet (NSW Office of Environment and Heritage)</dcterms:contributor>
      <skos:broader rdf:resource="http://104.244.76.201/Bionet-ANDS-test/schema/d1e81a1900"/>
      <skos:narrowMatch rdf:resource="http://104.244.76.201/Bionet-ANDS-test/vocab/reserve/d1e194a1900"/>
      <skos:narrowMatch rdf:resource="http://104.244.76.201/Bionet-ANDS-test/vocab/reserve/d1e195a1900"/>
      <skos:narrowMatch rdf:resource="http://104.244.76.201/Bionet-ANDS-test/vocab/reserve/d1e196a1900"/>
      <skos:narrowMatch rdf:resource="http://104.244.76.201/Bionet-ANDS-test/vocab/reserve/d1e197a1900"/>
      <skos:narrowMatch rdf:resource="http://104.244.76.201/Bionet-ANDS-test/vocab/reserve/d1e198a1900"/>
      <skos:narrowMatch rdf:resource="http://104.244.76.201/Bionet-ANDS-test/vocab/reserve/d1e199a1900"/>
      <skos:narrowMatch rdf:resource="http://104.244.76.201/Bionet-ANDS-test/vocab/reserve/d1e200a1900"/>
      <skos:definition xml:lang="en">If the record occurs within a reserve (as defined in the National Parks and Wildlife Act 1974) this field gives the name of that reserve. If the field is marked “N/”A, this indicates that the record does not occur within a reserve. The following types of reserve are covered under this legalisation:</skos:definition>
      <skos:definition xml:lang="en">Note: This field does not give the name of reserves administered under the Forestry Act 2012. See the ‘floraReserve’ field for information on flora reserves.</skos:definition>
      <skos:example xml:lang="en">“Cocoparra National Park”, “Bedooba State Conservation Area”</skos:example>
   </rdf:Description>

   <rdf:Description rdf:about="http://104.244.76.201/Bionet-ANDS-test/schema/d1e201a1900">
      <rdf:type rdf:resource="http://www.w3.org/2004/02/skos/core#Concept"/>
      <skos:prefLabel xml:lang="en">speciesFireDescription</skos:prefLabel>
      <dcterms:creator>Bionet (NSW Office of Environment and Heritage)</dcterms:creator>
      <dcterms:contributor>Bionet (NSW Office of Environment and Heritage)</dcterms:contributor>
      <skos:broader rdf:resource="http://104.244.76.201/Bionet-ANDS-test/schema/d1e81a1900"/>
      <skos:definition xml:lang="en">Information on any restrictions on the use of Controlled Burning as a Hazard Reduction Technique within 100m of the Occurrence record. Otherwise this field gives the value “N/A”</skos:definition>
      <skos:example xml:lang="en">“No burning within 100 metres of streams”, “No burning from 1 August to 31 March, and no more than once every 2 years. Retain logs on ground.”, “No fire”</skos:example>
   </rdf:Description>

   <rdf:Description rdf:about="http://104.244.76.201/Bionet-ANDS-test/schema/d1e206a1900">
      <rdf:type rdf:resource="http://www.w3.org/2004/02/skos/core#Concept"/>
      <skos:prefLabel xml:lang="en">stateForest</skos:prefLabel>
      <dcterms:creator>Bionet (NSW Office of Environment and Heritage)</dcterms:creator>
      <dcterms:contributor>Bionet (NSW Office of Environment and Heritage)</dcterms:contributor>
      <skos:broader rdf:resource="http://104.244.76.201/Bionet-ANDS-test/schema/d1e81a1900"/>
      <skos:definition xml:lang="en">If the record occurs within a state forest (as defined in the Forestry Act 2012) this field gives the name of that state forest. If the field is marked “N/A” this indicates that the record does not occur within a state forest.</skos:definition>
      <skos:example xml:lang="en">“Bom Bom State Forest”</skos:example>
   </rdf:Description>

   <rdf:Description rdf:about="http://104.244.76.201/Bionet-ANDS-test/schema/d1e211a1900">
      <rdf:type rdf:resource="http://www.w3.org/2004/02/skos/core#Concept"/>
      <skos:prefLabel xml:lang="en">vulnerability</skos:prefLabel>
      <dcterms:creator>Bionet (NSW Office of Environment and Heritage)</dcterms:creator>
      <dcterms:contributor>Bionet (NSW Office of Environment and Heritage)</dcterms:contributor>
      <skos:broader rdf:resource="http://104.244.76.201/Bionet-ANDS-test/schema/d1e81a1900"/>
      <skos:narrowMatch rdf:resource="http://104.244.76.201/Bionet-ANDS-test/vocab/vulnerability/d1e219a1900"/>
      <skos:narrowMatch rdf:resource="http://104.244.76.201/Bionet-ANDS-test/vocab/vulnerability/d1e220a1900"/>
      <skos:narrowMatch rdf:resource="http://104.244.76.201/Bionet-ANDS-test/vocab/vulnerability/d1e221a1900"/>
      <skos:narrowMatch rdf:resource="http://104.244.76.201/Bionet-ANDS-test/vocab/vulnerability/d1e222a1900"/>
      <skos:definition xml:lang="en">Vulnerability of the species to Hazard Reduction activities, based on a combination of Status on the Threatened Species Conservation Act and the species Geographic Extent as recorded in GeogExtent. Uses the following controlled vocabulary:</skos:definition>
      <skos:definition xml:lang="en">Otherwise this field gives the value “N/A”</skos:definition>
      <skos:example xml:lang="en">“VH”</skos:example>
   </rdf:Description>

   <rdf:Description rdf:about="http://104.244.76.201/Bionet-ANDS-test/schema/d1e414a1900">
      <rdf:type rdf:resource="http://www.w3.org/2004/02/skos/core#Concept"/>
      <skos:prefLabel xml:lang="en">reproductiveConditionFlora</skos:prefLabel>
      <dcterms:creator>Bionet (NSW Office of Environment and Heritage)</dcterms:creator>
      <dcterms:contributor>Bionet (NSW Office of Environment and Heritage)</dcterms:contributor>
      <skos:broader rdf:resource="http://104.244.76.201/Bionet-ANDS-test/schema/d1e409a1900"/>
      <skos:narrowMatch rdf:resource="http://104.244.76.201/Bionet-ANDS-test/vocab/reproductiveConditionFlora/d1e416a1900"/>
      <skos:narrowMatch rdf:resource="http://104.244.76.201/Bionet-ANDS-test/vocab/reproductiveConditionFlora/d1e417a1900"/>
      <skos:narrowMatch rdf:resource="http://104.244.76.201/Bionet-ANDS-test/vocab/reproductiveConditionFlora/d1e418a1900"/>
      <skos:narrowMatch rdf:resource="http://104.244.76.201/Bionet-ANDS-test/vocab/reproductiveConditionFlora/d1e419a1900"/>
      <skos:narrowMatch rdf:resource="http://104.244.76.201/Bionet-ANDS-test/vocab/reproductiveConditionFlora/d1e420a1900"/>
      <skos:narrowMatch rdf:resource="http://104.244.76.201/Bionet-ANDS-test/vocab/reproductiveConditionFlora/d1e421a1900"/>
      <skos:narrowMatch rdf:resource="http://104.244.76.201/Bionet-ANDS-test/vocab/reproductiveConditionFlora/d1e422a1900"/>
      <skos:narrowMatch rdf:resource="http://104.244.76.201/Bionet-ANDS-test/vocab/reproductiveConditionFlora/d1e423a1900"/>
   </rdf:Description>

   <rdf:Description rdf:about="http://104.244.76.201/Bionet-ANDS-test/schema/d1e424a1900">
      <rdf:type rdf:resource="http://www.w3.org/2004/02/skos/core#Concept"/>
      <skos:prefLabel xml:lang="en">reproductiveConditionFauna</skos:prefLabel>
      <dcterms:creator>Bionet (NSW Office of Environment and Heritage)</dcterms:creator>
      <dcterms:contributor>Bionet (NSW Office of Environment and Heritage)</dcterms:contributor>
      <skos:broader rdf:resource="http://104.244.76.201/Bionet-ANDS-test/schema/d1e409a1900"/>
      <skos:narrowMatch rdf:resource="http://104.244.76.201/Bionet-ANDS-test/vocab/reproductiveConditionFauna/d1e426a1900"/>
      <skos:narrowMatch rdf:resource="http://104.244.76.201/Bionet-ANDS-test/vocab/reproductiveConditionFauna/d1e427a1900"/>
      <skos:narrowMatch rdf:resource="http://104.244.76.201/Bionet-ANDS-test/vocab/reproductiveConditionFauna/d1e428a1900"/>
      <skos:narrowMatch rdf:resource="http://104.244.76.201/Bionet-ANDS-test/vocab/reproductiveConditionFauna/d1e429a1900"/>
      <skos:narrowMatch rdf:resource="http://104.244.76.201/Bionet-ANDS-test/vocab/reproductiveConditionFauna/d1e430a1900"/>
      <skos:narrowMatch rdf:resource="http://104.244.76.201/Bionet-ANDS-test/vocab/reproductiveConditionFauna/d1e431a1900"/>
      <skos:narrowMatch rdf:resource="http://104.244.76.201/Bionet-ANDS-test/vocab/reproductiveConditionFauna/d1e432a1900"/>
      <skos:narrowMatch rdf:resource="http://104.244.76.201/Bionet-ANDS-test/vocab/reproductiveConditionFauna/d1e433a1900"/>
      <skos:narrowMatch rdf:resource="http://104.244.76.201/Bionet-ANDS-test/vocab/reproductiveConditionFauna/d1e434a1900"/>
      <skos:narrowMatch rdf:resource="http://104.244.76.201/Bionet-ANDS-test/vocab/reproductiveConditionFauna/d1e435a1900"/>
      <skos:narrowMatch rdf:resource="http://104.244.76.201/Bionet-ANDS-test/vocab/reproductiveConditionFauna/d1e436a1900"/>
      <skos:narrowMatch rdf:resource="http://104.244.76.201/Bionet-ANDS-test/vocab/reproductiveConditionFauna/d1e438a1900"/>
      <skos:narrowMatch rdf:resource="http://104.244.76.201/Bionet-ANDS-test/vocab/reproductiveConditionFauna/d1e439a1900"/>
   </rdf:Description>

   <rdf:Description rdf:about="http://104.244.76.201/Bionet-ANDS-test/schema/d1e861a1900">
      <rdf:type rdf:resource="http://www.w3.org/2004/02/skos/core#Concept"/>
      <skos:prefLabel xml:lang="en">Aspect</skos:prefLabel>
      <dcterms:creator>Bionet (NSW Office of Environment and Heritage)</dcterms:creator>
      <dcterms:contributor>Bionet (NSW Office of Environment and Heritage)</dcterms:contributor>
      <skos:broader rdf:resource="http://104.244.76.201/Bionet-ANDS-test/schema/d1e843a1900"/>
      <skos:definition xml:lang="en">The aspect of the location where the observations was made measured in degrees clockwise from true North.</skos:definition>
      <skos:example xml:lang="en">“30”</skos:example>
   </rdf:Description>

   <rdf:Description rdf:about="http://104.244.76.201/Bionet-ANDS-test/schema/d1e866a1900">
      <rdf:type rdf:resource="http://www.w3.org/2004/02/skos/core#Concept"/>
      <skos:prefLabel xml:lang="en">Microhabitat</skos:prefLabel>
      <dcterms:creator>Bionet (NSW Office of Environment and Heritage)</dcterms:creator>
      <dcterms:contributor>Bionet (NSW Office of Environment and Heritage)</dcterms:contributor>
      <skos:broader rdf:resource="http://104.244.76.201/Bionet-ANDS-test/schema/d1e843a1900"/>
      <skos:narrowMatch rdf:resource="http://104.244.76.201/Bionet-ANDS-test/vocab/Microhabitat/d1e872a1900"/>
      <skos:narrowMatch rdf:resource="http://104.244.76.201/Bionet-ANDS-test/vocab/Microhabitat/d1e873a1900"/>
      <skos:narrowMatch rdf:resource="http://104.244.76.201/Bionet-ANDS-test/vocab/Microhabitat/d1e874a1900"/>
      <skos:narrowMatch rdf:resource="http://104.244.76.201/Bionet-ANDS-test/vocab/Microhabitat/d1e875a1900"/>
      <skos:narrowMatch rdf:resource="http://104.244.76.201/Bionet-ANDS-test/vocab/Microhabitat/d1e876a1900"/>
      <skos:narrowMatch rdf:resource="http://104.244.76.201/Bionet-ANDS-test/vocab/Microhabitat/d1e877a1900"/>
      <skos:narrowMatch rdf:resource="http://104.244.76.201/Bionet-ANDS-test/vocab/Microhabitat/d1e878a1900"/>
      <skos:narrowMatch rdf:resource="http://104.244.76.201/Bionet-ANDS-test/vocab/Microhabitat/d1e879a1900"/>
      <skos:narrowMatch rdf:resource="http://104.244.76.201/Bionet-ANDS-test/vocab/Microhabitat/d1e880a1900"/>
      <skos:narrowMatch rdf:resource="http://104.244.76.201/Bionet-ANDS-test/vocab/Microhabitat/d1e881a1900"/>
      <skos:narrowMatch rdf:resource="http://104.244.76.201/Bionet-ANDS-test/vocab/Microhabitat/d1e882a1900"/>
      <skos:narrowMatch rdf:resource="http://104.244.76.201/Bionet-ANDS-test/vocab/Microhabitat/d1e884a1900"/>
      <skos:narrowMatch rdf:resource="http://104.244.76.201/Bionet-ANDS-test/vocab/Microhabitat/d1e885a1900"/>
      <skos:narrowMatch rdf:resource="http://104.244.76.201/Bionet-ANDS-test/vocab/Microhabitat/d1e886a1900"/>
      <skos:narrowMatch rdf:resource="http://104.244.76.201/Bionet-ANDS-test/vocab/Microhabitat/d1e887a1900"/>
      <skos:narrowMatch rdf:resource="http://104.244.76.201/Bionet-ANDS-test/vocab/Microhabitat/d1e888a1900"/>
      <skos:narrowMatch rdf:resource="http://104.244.76.201/Bionet-ANDS-test/vocab/Microhabitat/d1e889a1900"/>
      <skos:narrowMatch rdf:resource="http://104.244.76.201/Bionet-ANDS-test/vocab/Microhabitat/d1e890a1900"/>
      <skos:narrowMatch rdf:resource="http://104.244.76.201/Bionet-ANDS-test/vocab/Microhabitat/d1e891a1900"/>
      <skos:narrowMatch rdf:resource="http://104.244.76.201/Bionet-ANDS-test/vocab/Microhabitat/d1e892a1900"/>
      <skos:narrowMatch rdf:resource="http://104.244.76.201/Bionet-ANDS-test/vocab/Microhabitat/d1e893a1900"/>
      <skos:narrowMatch rdf:resource="http://104.244.76.201/Bionet-ANDS-test/vocab/Microhabitat/d1e894a1900"/>
      <skos:narrowMatch rdf:resource="http://104.244.76.201/Bionet-ANDS-test/vocab/Microhabitat/d1e896a1900"/>
      <skos:narrowMatch rdf:resource="http://104.244.76.201/Bionet-ANDS-test/vocab/Microhabitat/d1e897a1900"/>
      <skos:narrowMatch rdf:resource="http://104.244.76.201/Bionet-ANDS-test/vocab/Microhabitat/d1e898a1900"/>
      <skos:narrowMatch rdf:resource="http://104.244.76.201/Bionet-ANDS-test/vocab/Microhabitat/d1e899a1900"/>
      <skos:narrowMatch rdf:resource="http://104.244.76.201/Bionet-ANDS-test/vocab/Microhabitat/d1e900a1900"/>
      <skos:narrowMatch rdf:resource="http://104.244.76.201/Bionet-ANDS-test/vocab/Microhabitat/d1e901a1900"/>
      <skos:narrowMatch rdf:resource="http://104.244.76.201/Bionet-ANDS-test/vocab/Microhabitat/d1e902a1900"/>
      <skos:narrowMatch rdf:resource="http://104.244.76.201/Bionet-ANDS-test/vocab/Microhabitat/d1e903a1900"/>
      <skos:narrowMatch rdf:resource="http://104.244.76.201/Bionet-ANDS-test/vocab/Microhabitat/d1e904a1900"/>
      <skos:narrowMatch rdf:resource="http://104.244.76.201/Bionet-ANDS-test/vocab/Microhabitat/d1e905a1900"/>
      <skos:narrowMatch rdf:resource="http://104.244.76.201/Bionet-ANDS-test/vocab/Microhabitat/d1e906a1900"/>
      <skos:narrowMatch rdf:resource="http://104.244.76.201/Bionet-ANDS-test/vocab/Microhabitat/d1e908a1900"/>
      <skos:narrowMatch rdf:resource="http://104.244.76.201/Bionet-ANDS-test/vocab/Microhabitat/d1e909a1900"/>
      <skos:narrowMatch rdf:resource="http://104.244.76.201/Bionet-ANDS-test/vocab/Microhabitat/d1e910a1900"/>
      <skos:narrowMatch rdf:resource="http://104.244.76.201/Bionet-ANDS-test/vocab/Microhabitat/d1e911a1900"/>
      <skos:narrowMatch rdf:resource="http://104.244.76.201/Bionet-ANDS-test/vocab/Microhabitat/d1e912a1900"/>
      <skos:narrowMatch rdf:resource="http://104.244.76.201/Bionet-ANDS-test/vocab/Microhabitat/d1e913a1900"/>
      <skos:definition xml:lang="en">The small-scale habitat (e.g. on ground, or in tree) as per the following controlled vocabulary:</skos:definition>
      <skos:example xml:lang="en">“In burrow”</skos:example>
   </rdf:Description>

   <rdf:Description rdf:about="http://104.244.76.201/Bionet-ANDS-test/schema/d1e914a1900">
      <rdf:type rdf:resource="http://www.w3.org/2004/02/skos/core#Concept"/>
      <skos:prefLabel xml:lang="en">Slope</skos:prefLabel>
      <dcterms:creator>Bionet (NSW Office of Environment and Heritage)</dcterms:creator>
      <dcterms:contributor>Bionet (NSW Office of Environment and Heritage)</dcterms:contributor>
      <skos:broader rdf:resource="http://104.244.76.201/Bionet-ANDS-test/schema/d1e843a1900"/>
      <skos:definition xml:lang="en">The slope of the location where the observation was made measured in degrees from horizontal</skos:definition>
      <skos:example xml:lang="en">“15”</skos:example>
   </rdf:Description>

   <rdf:Description rdf:about="http://104.244.76.201/Bionet-ANDS-test/schema/d1e919a1900">
      <rdf:type rdf:resource="http://www.w3.org/2004/02/skos/core#Concept"/>
      <skos:prefLabel xml:lang="en">SurfaceGeology</skos:prefLabel>
      <dcterms:creator>Bionet (NSW Office of Environment and Heritage)</dcterms:creator>
      <dcterms:contributor>Bionet (NSW Office of Environment and Heritage)</dcterms:contributor>
      <skos:broader rdf:resource="http://104.244.76.201/Bionet-ANDS-test/schema/d1e843a1900"/>
      <skos:narrowMatch rdf:resource="http://104.244.76.201/Bionet-ANDS-test/vocab/SurfaceGeology/d1e925a1900"/>
      <skos:narrowMatch rdf:resource="http://104.244.76.201/Bionet-ANDS-test/vocab/SurfaceGeology/d1e926a1900"/>
      <skos:narrowMatch rdf:resource="http://104.244.76.201/Bionet-ANDS-test/vocab/SurfaceGeology/d1e927a1900"/>
      <skos:narrowMatch rdf:resource="http://104.244.76.201/Bionet-ANDS-test/vocab/SurfaceGeology/d1e928a1900"/>
      <skos:narrowMatch rdf:resource="http://104.244.76.201/Bionet-ANDS-test/vocab/SurfaceGeology/d1e929a1900"/>
      <skos:narrowMatch rdf:resource="http://104.244.76.201/Bionet-ANDS-test/vocab/SurfaceGeology/d1e930a1900"/>
      <skos:narrowMatch rdf:resource="http://104.244.76.201/Bionet-ANDS-test/vocab/SurfaceGeology/d1e931a1900"/>
      <skos:narrowMatch rdf:resource="http://104.244.76.201/Bionet-ANDS-test/vocab/SurfaceGeology/d1e932a1900"/>
      <skos:narrowMatch rdf:resource="http://104.244.76.201/Bionet-ANDS-test/vocab/SurfaceGeology/d1e933a1900"/>
      <skos:narrowMatch rdf:resource="http://104.244.76.201/Bionet-ANDS-test/vocab/SurfaceGeology/d1e934a1900"/>
      <skos:narrowMatch rdf:resource="http://104.244.76.201/Bionet-ANDS-test/vocab/SurfaceGeology/d1e935a1900"/>
      <skos:narrowMatch rdf:resource="http://104.244.76.201/Bionet-ANDS-test/vocab/SurfaceGeology/d1e937a1900"/>
      <skos:narrowMatch rdf:resource="http://104.244.76.201/Bionet-ANDS-test/vocab/SurfaceGeology/d1e938a1900"/>
      <skos:narrowMatch rdf:resource="http://104.244.76.201/Bionet-ANDS-test/vocab/SurfaceGeology/d1e939a1900"/>
      <skos:narrowMatch rdf:resource="http://104.244.76.201/Bionet-ANDS-test/vocab/SurfaceGeology/d1e940a1900"/>
      <skos:narrowMatch rdf:resource="http://104.244.76.201/Bionet-ANDS-test/vocab/SurfaceGeology/d1e941a1900"/>
      <skos:narrowMatch rdf:resource="http://104.244.76.201/Bionet-ANDS-test/vocab/SurfaceGeology/d1e942a1900"/>
      <skos:narrowMatch rdf:resource="http://104.244.76.201/Bionet-ANDS-test/vocab/SurfaceGeology/d1e943a1900"/>
      <skos:narrowMatch rdf:resource="http://104.244.76.201/Bionet-ANDS-test/vocab/SurfaceGeology/d1e944a1900"/>
      <skos:narrowMatch rdf:resource="http://104.244.76.201/Bionet-ANDS-test/vocab/SurfaceGeology/d1e945a1900"/>
      <skos:narrowMatch rdf:resource="http://104.244.76.201/Bionet-ANDS-test/vocab/SurfaceGeology/d1e946a1900"/>
      <skos:narrowMatch rdf:resource="http://104.244.76.201/Bionet-ANDS-test/vocab/SurfaceGeology/d1e947a1900"/>
      <skos:narrowMatch rdf:resource="http://104.244.76.201/Bionet-ANDS-test/vocab/SurfaceGeology/d1e949a1900"/>
      <skos:narrowMatch rdf:resource="http://104.244.76.201/Bionet-ANDS-test/vocab/SurfaceGeology/d1e950a1900"/>
      <skos:narrowMatch rdf:resource="http://104.244.76.201/Bionet-ANDS-test/vocab/SurfaceGeology/d1e951a1900"/>
      <skos:narrowMatch rdf:resource="http://104.244.76.201/Bionet-ANDS-test/vocab/SurfaceGeology/d1e952a1900"/>
      <skos:narrowMatch rdf:resource="http://104.244.76.201/Bionet-ANDS-test/vocab/SurfaceGeology/d1e953a1900"/>
      <skos:narrowMatch rdf:resource="http://104.244.76.201/Bionet-ANDS-test/vocab/SurfaceGeology/d1e954a1900"/>
      <skos:narrowMatch rdf:resource="http://104.244.76.201/Bionet-ANDS-test/vocab/SurfaceGeology/d1e955a1900"/>
      <skos:narrowMatch rdf:resource="http://104.244.76.201/Bionet-ANDS-test/vocab/SurfaceGeology/d1e956a1900"/>
      <skos:narrowMatch rdf:resource="http://104.244.76.201/Bionet-ANDS-test/vocab/SurfaceGeology/d1e957a1900"/>
      <skos:narrowMatch rdf:resource="http://104.244.76.201/Bionet-ANDS-test/vocab/SurfaceGeology/d1e958a1900"/>
      <skos:narrowMatch rdf:resource="http://104.244.76.201/Bionet-ANDS-test/vocab/SurfaceGeology/d1e959a1900"/>
      <skos:narrowMatch rdf:resource="http://104.244.76.201/Bionet-ANDS-test/vocab/SurfaceGeology/d1e961a1900"/>
      <skos:narrowMatch rdf:resource="http://104.244.76.201/Bionet-ANDS-test/vocab/SurfaceGeology/d1e962a1900"/>
      <skos:narrowMatch rdf:resource="http://104.244.76.201/Bionet-ANDS-test/vocab/SurfaceGeology/d1e963a1900"/>
      <skos:narrowMatch rdf:resource="http://104.244.76.201/Bionet-ANDS-test/vocab/SurfaceGeology/d1e964a1900"/>
      <skos:narrowMatch rdf:resource="http://104.244.76.201/Bionet-ANDS-test/vocab/SurfaceGeology/d1e965a1900"/>
      <skos:narrowMatch rdf:resource="http://104.244.76.201/Bionet-ANDS-test/vocab/SurfaceGeology/d1e966a1900"/>
      <skos:narrowMatch rdf:resource="http://104.244.76.201/Bionet-ANDS-test/vocab/SurfaceGeology/d1e967a1900"/>
      <skos:narrowMatch rdf:resource="http://104.244.76.201/Bionet-ANDS-test/vocab/SurfaceGeology/d1e968a1900"/>
      <skos:narrowMatch rdf:resource="http://104.244.76.201/Bionet-ANDS-test/vocab/SurfaceGeology/d1e969a1900"/>
      <skos:narrowMatch rdf:resource="http://104.244.76.201/Bionet-ANDS-test/vocab/SurfaceGeology/d1e970a1900"/>
      <skos:narrowMatch rdf:resource="http://104.244.76.201/Bionet-ANDS-test/vocab/SurfaceGeology/d1e971a1900"/>
      <skos:narrowMatch rdf:resource="http://104.244.76.201/Bionet-ANDS-test/vocab/SurfaceGeology/d1e973a1900"/>
      <skos:narrowMatch rdf:resource="http://104.244.76.201/Bionet-ANDS-test/vocab/SurfaceGeology/d1e974a1900"/>
      <skos:narrowMatch rdf:resource="http://104.244.76.201/Bionet-ANDS-test/vocab/SurfaceGeology/d1e975a1900"/>
      <skos:narrowMatch rdf:resource="http://104.244.76.201/Bionet-ANDS-test/vocab/SurfaceGeology/d1e976a1900"/>
      <skos:narrowMatch rdf:resource="http://104.244.76.201/Bionet-ANDS-test/vocab/SurfaceGeology/d1e977a1900"/>
      <skos:narrowMatch rdf:resource="http://104.244.76.201/Bionet-ANDS-test/vocab/SurfaceGeology/d1e978a1900"/>
      <skos:narrowMatch rdf:resource="http://104.244.76.201/Bionet-ANDS-test/vocab/SurfaceGeology/d1e979a1900"/>
      <skos:narrowMatch rdf:resource="http://104.244.76.201/Bionet-ANDS-test/vocab/SurfaceGeology/d1e980a1900"/>
      <skos:narrowMatch rdf:resource="http://104.244.76.201/Bionet-ANDS-test/vocab/SurfaceGeology/d1e981a1900"/>
      <skos:narrowMatch rdf:resource="http://104.244.76.201/Bionet-ANDS-test/vocab/SurfaceGeology/d1e982a1900"/>
      <skos:narrowMatch rdf:resource="http://104.244.76.201/Bionet-ANDS-test/vocab/SurfaceGeology/d1e983a1900"/>
      <skos:narrowMatch rdf:resource="http://104.244.76.201/Bionet-ANDS-test/vocab/SurfaceGeology/d1e985a1900"/>
      <skos:narrowMatch rdf:resource="http://104.244.76.201/Bionet-ANDS-test/vocab/SurfaceGeology/d1e986a1900"/>
      <skos:narrowMatch rdf:resource="http://104.244.76.201/Bionet-ANDS-test/vocab/SurfaceGeology/d1e987a1900"/>
      <skos:narrowMatch rdf:resource="http://104.244.76.201/Bionet-ANDS-test/vocab/SurfaceGeology/d1e988a1900"/>
      <skos:narrowMatch rdf:resource="http://104.244.76.201/Bionet-ANDS-test/vocab/SurfaceGeology/d1e989a1900"/>
      <skos:narrowMatch rdf:resource="http://104.244.76.201/Bionet-ANDS-test/vocab/SurfaceGeology/d1e990a1900"/>
      <skos:narrowMatch rdf:resource="http://104.244.76.201/Bionet-ANDS-test/vocab/SurfaceGeology/d1e991a1900"/>
      <skos:narrowMatch rdf:resource="http://104.244.76.201/Bionet-ANDS-test/vocab/SurfaceGeology/d1e992a1900"/>
      <skos:narrowMatch rdf:resource="http://104.244.76.201/Bionet-ANDS-test/vocab/SurfaceGeology/d1e993a1900"/>
      <skos:narrowMatch rdf:resource="http://104.244.76.201/Bionet-ANDS-test/vocab/SurfaceGeology/d1e994a1900"/>
      <skos:definition xml:lang="en">The surface geology of the location where the observation was made as per the following controlled vocabulary:</skos:definition>
      <skos:example xml:lang="en">“Basalt”</skos:example>
   </rdf:Description>

</rdf:RDF>
